finished polishing proof

Infrastructure.v
@@ -1,9 +1,10 @@
 Require Import Logic.FunctionalExtensionality.
 Require Import Lia.
+Require Import PeanoNat.
 From LSEH Require Import RelConfig.
 Import Lists.List. Import ListNotations.
-Import Strings.String. Import LexiToSalt.
-Import Lexi. Import Salt.
+Import Strings.String. Import LexaToSalt.
+Import Lexa. Import Salt.
 Ltac trysolve :=
   try easy;try discriminate;
   try congruence;try tauto;
@@ -16,32 +17,6 @@ Ltac super_a :=
 (* ---------------------------------------------------------
    ------------------ Lemmas for Salt ----------------------
    --------------------------------------------------------- *)
-Theorem reg_file_front_update : forall (R:reg_file) a v1 v2
-  oi os o1 o2 o3 o4 o5 o6,
-  (a = ip \/ a = sp \/ a = nat_reg 1 \/ a = nat_reg 2 \/
-   a = nat_reg 3 \/ a = nat_reg 4 \/ a = nat_reg 5
-   \/ a = nat_reg 6) ->
-  R = [(ip,oi);(sp,os);(nat_reg 1,o1);(nat_reg 2,o2);(nat_reg 3,o3);
-      (nat_reg 4,o4);(nat_reg 5,o5);(nat_reg 6,o6)] ->
-  (a !->r v1; a !->r v2; R) = (a !->r v1; R).
-Proof. intros. repeat (destruct H;super_a). Qed.
-Theorem reg_file_swap : forall R a b v1 v2
-  oi os o1 o2 o3 o4 o5 o6,
-  (a = ip \/ a = sp \/ a = nat_reg 1 \/ a = nat_reg 2 \/
-   a = nat_reg 3 \/ a = nat_reg 4 \/ a = nat_reg 5
-   \/ a = nat_reg 6) ->
-  (b = ip \/ b = sp \/ b = nat_reg 1 \/ b = nat_reg 2 \/
-   b = nat_reg 3 \/ b = nat_reg 4 \/ b = nat_reg 5
-   \/ b = nat_reg 6) ->
-  reg_eqb a b = false ->
-  R = [(ip,oi);(sp,os);(nat_reg 1,o1);(nat_reg 2,o2);(nat_reg 3,o3);
-      (nat_reg 4,o4);(nat_reg 5,o5);(nat_reg 6,o6)] ->
-  (a !->r v1; b !->r v2; R) = (b !->r v2; a !->r v1; R).
-Proof with super_a.
-  intros. subst.
-  repeat (destruct H as [ | ]);
-  repeat (destruct H0 as [ | ])...
-Qed.
 Lemma h_eqb_refl : forall (a:heap_loc), a = a -> h_eqb a a = true.
 Proof. intros. unfold h_eqb. destruct a. apply PeanoNat.Nat.eqb_refl. Qed.
 Lemma c_eqb_refl : forall (a:code_loc), a = a -> c_eqb a a = true.
@@ -53,3 +28,562 @@ Proof with super_a.
   intros. unfold th_update. extensionality x. destruct (h_eqb a x)...
 Qed.
 
+(* ---------------------------------------------------------
+                       Some Useful Lemmas for
+                     Proving Condition 1 and 3
+   --------------------------------------------------------- *)
+Lemma one_eval_ctx_rel :
+  forall frm frm_lst C_mem L,
+    (LS_rel_hdl L frm frm_lst
+     /\ is_h_frm_general_hdl frm = true)
+    <->
+    LS_rel_eval_ctx C_mem [hdl_led_lst frm []]
+      [(hloc_num L,stack frm_lst)].
+Proof with super_a.
+  intros. split.
+  - intros.
+    apply rel_eval_ctx_lst with
+      (K:=hdl_led_lst frm [])...
+    apply rel_hdl_stk_base with
+      (Flst:=[]) (s:=[])...
+  - intros. split;
+      inversion H;subst;
+      inversion H5;subst;
+      inversion H7...
+    inversion H3...
+Qed.
+Lemma length_ctx_stk :
+  forall C_mem H K,
+    LS_rel_eval_ctx C_mem K H ->
+    List.length H <= List.length K.
+Proof with super_a.
+  intros C_mem H.
+  induction H...
+  intros. inversion H0;subst.
+  apply IHlist in H4.
+  apply le_n_S in H4.
+  rewrite H4. cbn...
+Qed.
+(* ---------------------------------------------------------
+   ------ Some Basic Lemmas for Proving Condition 3 --------
+   --------------------------------------------------------- *)
+Lemma term_trans_not_nil : forall tm,
+    term_trans tm <> [].
+Proof with automate.
+  intros. unfold not. destruct tm;simpl...
+  destruct e;intros;simpl;apply eq_sym in H;
+    generalize dependent H...
+  - apply app_cons_not_nil.
+  - destruct a...
+Qed.
+Lemma ins_verify : forall (A : Type) (l l' : list A) (d : A) (n : nat),
+    nth (n + List.length l) (l ++ l') d = nth n l' d.
+Proof.
+  intros. rewrite PeanoNat.Nat.add_comm.
+  apply app_nth2_plus.
+Qed.
+Lemma val_dir_trans_var_deref : forall E (v:value) lst,
+    (forall ind:nat, v = ind_val ind -> ind < List.length E) ->
+    val_direct_trans v (List.map run_cst_trans E ++ lst)
+    = run_cst_trans (L.var_deref E v).
+Proof with super_a.
+  intros. destruct v as [|[]]...
+  rewrite <- map_nth with (d:=L.ns)...
+  rewrite app_nth1... specialize H with n.
+  rewrite map_length...  
+Qed.
+
+Lemma stk_points_to_preserves :
+  forall s s' L' s_added,
+    3 < List.length s ->
+    stk_points_to s s' L' <->
+    stk_points_to (s_added ++ s) s' L'.
+Proof with super_a.
+  unfold stk_points_to.
+  intros. split;intros;
+    rewrite <- H0;
+    rewrite rev_app_distr with (y:=s);
+    rewrite nth_error_app1;super_a;
+    rewrite rev_length...    
+Qed.
+
+(* ---------------------------------------------------------
+                   Lemmas for Working with 
+            Evaluation Context and Continuations
+   --------------------------------------------------------- *)
+Definition get_hdl_lab (hdl_frm_lst:hdl_led_frm_lst) : nat :=
+  match hdl_frm_lst with
+  | hdl_led_lst (hdl_f (hdl_lab L) _ _ _) _ => L
+  end.
+Definition frm_to_hloc frm :=
+  hloc_num (get_hdl_lab frm).
+Definition is_hdllst_general hdl_lst:=
+  match hdl_lst with
+  | hdl_led_lst frm alst =>
+      is_h_frm_general_hdl frm
+  end.
+Lemma last_eval_ctx_rel :
+  forall s L frm C_mem Ks H,
+    LS_rel_eval_ctx C_mem
+      (Ks ++ [frm])
+      (H ++ [(hloc_num L,stack s)]) ->
+    is_hdllst_general frm = true ->
+    LS_rel_hdl_stk C_mem L
+      frm (stack s)
+    /\ L = get_hdl_lab frm.
+Proof with super_a.
+  intros.
+  destruct frm as
+    [[[L_h] L_env lab_op []] alst];
+    trysolve.
+  generalize dependent H.
+  induction Ks.
+  - intros.
+    destruct H.
+    2:{ apply length_ctx_stk in H0.
+        rewrite app_length in H0.
+        rewrite Nat.add_comm in H0.
+        cbn in H0... }
+    inversion H0...
+    inversion H8...
+    inversion H5...
+  - intros. inversion H0;subst.
+    destruct H;inversion H5;
+      subst;trysolve.
+    inversion H6.
+    destruct Ks...
+Qed.
+Lemma eval_ctx_app_split :
+  forall C_mem K' K H,
+    LS_rel_eval_ctx C_mem
+      (K' ++ K) H ->
+    exists H_ld H_ed,
+      LS_rel_eval_ctx C_mem K' H_ld
+      /\ LS_rel_eval_ctx C_mem K H_ed
+      /\ H = H_ld ++ H_ed.
+Proof with super_a.
+  intros. generalize dependent H.
+  induction K'.
+  { intros.
+    exists sh_empty,H... }
+  intros. inversion H0...
+  apply IHK' in H4.
+  destruct H4 as
+    [H_ld [H_ed [hyp1 [hyp2 hyp3]]]].
+  exists ((hloc_num L,stack s)
+            :: H_ld),H_ed...
+  intros. eapply H7...
+Qed.
+Lemma eval_ctx_last_label :
+  forall C_mem H K' L frm,
+    LS_rel_eval_ctx C_mem
+      (K' ++ [frm]) H ->
+    is_hdllst_general frm = true ->
+    L = get_hdl_lab frm ->
+    exists H' s,
+      H = H' ++ [(hloc_num L,
+                   stack s)]
+      /\ 1 < List.length s.
+Proof with super_a.
+  intros.
+  destruct frm as
+    [[[L_h] L_env lab_op []] alst]...
+  generalize dependent H.
+  induction K'.
+  { intros. 
+    inversion H0...
+    exists sh_empty,s.
+    apply length_ctx_stk in H0.
+    inversion H5;inversion H6;
+    inversion H10...
+    rewrite app_length... }
+  intros. inversion H0...
+  apply IHK' in H5.
+  destruct H5 as [H' [s' [h1 h2]]].
+  exists ((hloc_num L, stack s) :: H'),s'...
+Qed.
+
+Lemma eval_ctx_app_comp :
+  forall C_mem K' K H_ld H_ed,
+    LS_rel_eval_ctx C_mem K' H_ld ->
+    LS_rel_eval_ctx C_mem K H_ed ->
+    (forall H_ld' H_ed' L s L' s',
+        H_ld = H_ld' ++ [(L,stack s)] ->
+        H_ed = (L',stack s') :: H_ed' ->
+        stk_points_to s s' L') ->
+    LS_rel_eval_ctx C_mem
+      (K' ++ K) (H_ld ++ H_ed).
+Proof with super_a.
+  intros. generalize dependent H_ld.
+  induction K'.
+  { intros. inversion H... }
+  destruct H_ed as [|b H_ed']eqn:?.
+  { intros. inversion H0...
+    repeat (rewrite app_nil_r)... }
+  intros. inversion H;subst.
+  pose proof H5 as H5_backup.
+  apply IHK' in H5.
+  { constructor...
+    intros.
+    destruct H2.
+    - (*destructing it means we prove the first of H_ed
+        is the s_pr ev of Hld*)
+      inversion H5_backup...
+      inversion H3...
+      specialize H1 with
+        (H_ld':=[]) (H_ed':=H')
+        (L:=hloc_num L) (s:=s).
+      assert (Tmp:[(L, stack s)] = [(L, stack s)])...
+    - inversion H3... }
+  (*also use H1 here *)
+  intros. inversion H4...
+  apply H1 with
+    (H_ld':=(hloc_num L,stack s)
+              :: H_ld')
+    (H_ed':=H_ed'0) (L:=L0)...
+Qed.
+Lemma eval_ctx_app_2_middle :
+  forall C_mem K K' frm1 frm2 H,
+    LS_rel_eval_ctx C_mem
+      (K' ++ frm1 :: frm2 :: K) H ->
+    is_hdllst_general frm1 = true ->
+    is_hdllst_general frm2 = true ->
+    exists s1 s2 H_ld H_ed,
+      LS_rel_eval_ctx C_mem (K' ++ [frm1])
+        (H_ld ++ [(frm_to_hloc frm1,stack s1)])
+      /\ LS_rel_eval_ctx C_mem (frm2 :: K)
+           ((frm_to_hloc frm2,stack s2) :: H_ed)
+      /\ H = H_ld ++ (frm_to_hloc frm1,stack s1)
+               :: (frm_to_hloc frm2,stack s2) :: H_ed
+      /\ stk_points_to s1 s2 (frm_to_hloc frm2).
+Proof with super_a.
+  intros. generalize dependent H.
+  induction K'.
+  { intros. inversion H0...
+    inversion H6...
+    exists s,s0,sh_empty,H.
+    inversion H7;subst;
+    inversion H5;subst;
+    inversion H10;subst;
+    inversion H14... }
+  intros. inversion H0...
+  apply IHK' in H6.
+  destruct H6 as
+    [s1 [s2 [H_ld [H_ed hyp]]]].
+  destruct hyp as [hyp1 [hyp2 [hyp3 hyp4]]].
+  exists s1,s2,((hloc_num L,stack s)
+                  :: H_ld),H_ed...
+  intros. destruct H_ld;inversion H...
+  - eapply H9...
+  - eapply H9...
+Qed.
+Lemma app_inv_length_ld :
+  forall {A:Type} (l1 l2 l3 l4:list A),
+    l1 ++ l2 = l3 ++ l4 ->
+    List.length l2 = 5 ->
+    List.length l4 = 5->
+    l1 = l3.
+Proof with super_a.
+  intros.
+  assert (forall {A:Type} (l1 l2:list A),
+             l1 = l2 -> List.length l1
+                        = List.length l2)...
+  pose proof H as H3.
+  apply H2 in H3.
+  apply app_inv_tail with (l:=l2).
+  repeat (rewrite app_length in H3).
+  repeat (destruct l2 as [|];super_a).
+  repeat (destruct l4 as [|];super_a).
+  rewrite H. generalize dependent l1.
+  induction l3...
+  - destruct l1...
+  - intros. destruct l1.
+    + inversion H3...
+    + rewrite IHl3 with
+        (l1:=l1)...
+      inversion H...
+Qed.
+Lemma app_inv_length_ed :
+  forall {A:Type} (l1 l2 l3 l4:list A),
+    l1 ++ l2 = l3 ++ l4 ->
+    List.length l2 = 5 ->
+    List.length l4 = 5->
+    l2 = l4.
+Proof with super_a.
+  intros.
+  pose proof H.
+  apply app_inv_length_ld in H...
+  eapply app_inv_head...
+Qed.
+Lemma eval_ctx_last_points_to_preserves :
+  forall C_mem K H L s frmlst1 frmlst2 frm alst,
+    LS_rel_eval_ctx C_mem
+      (K ++ [hdl_led_lst frm alst])  
+      (H ++ [(hloc_num L, stack (s ++ frmlst1))]) ->
+    LS_rel_hdl L frm frmlst1 ->
+    LS_rel_hdl L frm frmlst2 ->
+    LS_rel_eval_ctx C_mem
+      (K ++ [hdl_led_lst frm alst])  
+      (H ++ [(hloc_num L, stack (s ++ frmlst2))]).
+Proof with super_a.
+  intros. inversion H1...
+  inversion H2...
+  generalize dependent K.
+  induction H...
+  - intros.
+    inversion H0...
+    inversion H8...
+    inversion H5...
+    + apply app_inv_length_ld
+        in H...
+    + inversion H5...
+      apply app_inv_length_ed
+        in H...
+  - intros.
+    destruct K;
+      inversion H0;subst.
+    { inversion H8.
+      destruct H... }
+    apply IHlist in H8.
+    constructor...
+    destruct H. 
+    + intros. 
+      inversion H...
+      unfold stk_points_to.
+      rewrite app_length.
+      assert (stk_points_to s0
+                (s ++
+                   [loc_w (cloc handle_loc 10);
+                    loc_w (hloc L_prev (Datatypes.length s_prev));
+                    int_w 0; 
+                    loc_w (hloc L_env 0);
+                    loc_w (cloc Clab_op 0)]) L).
+      { apply H10 with (H':=[])... }
+      unfold stk_points_to in H3.
+      rewrite app_length in H3...
+    + intros. inversion H3...
+      apply H10 with
+        (H':=H ++
+               [(hloc_num L,
+                  stack (s ++
+                           [loc_w (cloc handle_loc 10);
+                            loc_w (hloc L_prev (Datatypes.length s_prev));
+                            int_w 0; 
+                            loc_w (hloc L_env 0);
+                            loc_w (cloc Clab_op 0)]))])...
+Qed.
+
+Lemma app_inv_last :
+  forall {A:Type} (l1:list A) l2 a b,
+    l1 ++ [a] = l2 ++ [b] ->
+    a = b
+    /\ l1 = l2.
+Proof with super_a.
+  intros. generalize dependent l2.
+  induction l1.
+  - intros.
+    induction l2...
+    + inversion H...
+    + inversion H...
+      induction l2...
+    + induction l2...
+  - intros.
+    induction l2.
+    + induction l1...
+    + split.
+      * apply IHl1 with
+          (l2:=l2).
+        inversion H...
+      * inversion H...
+        apply IHl1 in H2.
+        destruct H2.
+        rewrite H1...
+Qed.
+
+Lemma update_nth_one_iter :
+  forall {A} n a lst (v:A),
+    update_nth (S n) (a :: lst) v = a :: update_nth n lst v.
+Proof. intros. super_a. Qed.
+Lemma update_nth_split :
+  forall {A} l1 l2 n (v:A),
+    n <= Datatypes.length l2 ->
+    update_nth (List.length (l1 ++ l2) - n) (l1 ++ l2) v
+    = l1 ++ update_nth (List.length l2 - n) l2 v.
+Proof with super_a.
+  intros. induction l1;automate.
+  assert (List.length ((a :: l1) ++ l2)
+            = S (List.length (l1 ++ l2)));
+    automate. rewrite H0.
+  rewrite Nat.sub_succ_l.
+  2:{ rewrite app_length... }
+  rewrite <- app_comm_cons.
+  rewrite update_nth_one_iter...
+Qed.
+Lemma update_nth_length :
+  forall {A} n l (v:A),
+    List.length (update_nth n l v)
+    = List.length l.
+Proof with super_a.
+  intros. generalize dependent n.
+  induction l;destruct n...
+Qed.
+Lemma tup_heap_nil_split :
+  forall H1 H2 L,
+    th_comp H1 H2 L = tuple [] ->
+    H1 L = tuple [] /\ H2 L = tuple [].
+Proof with super_a.
+  intros. split;
+    unfold th_comp in H;
+    destruct (H1 L) as []eqn:?;
+                         destruct l...
+Qed.
+Lemma th_comp_comm_th_update :
+  forall x v H1 H2,
+    H2 x = tuple [] ->
+    th_comp (x !->t v; H1) H2 =
+      (x !->t v; th_comp H1 H2).
+Proof with super_a.
+  intros. extensionality x'.
+  unfold th_comp,th_update,
+    h_eqb. destruct x as [x],x' as [x'].
+  destruct (x =? x') as []eqn:?...
+  rewrite Nat.eqb_eq in Heqb.
+  destruct v as [[|]]...
+Qed.
+Lemma cont_heap_split :
+  forall C_mem LH_cont_ld LH_cont_ed
+         SH_cont SH_ctup,
+    (*L_last is label of last stack
+      in the Ks*)
+    LS_rel_cont_heap C_mem
+      (LH_cont_ld ++ LH_cont_ed)
+      (SH_cont,SH_ctup) ->
+    exists SH_cont_ld SH_cont_ed
+           SH_ctup_ld SH_ctup_ed,
+      LS_rel_cont_heap C_mem LH_cont_ld
+        (SH_cont_ld,SH_ctup_ld)
+      /\ LS_rel_cont_heap C_mem LH_cont_ed
+           (SH_cont_ed,SH_ctup_ed)
+      /\ SH_cont = SH_cont_ld ++ SH_cont_ed
+      /\ SH_ctup = th_comp SH_ctup_ld SH_ctup_ed
+      /\ (forall L,
+             SH_ctup_ed L = tuple []
+             \/ SH_ctup_ld L = tuple []).
+(*can't both be non nil.
+if ed not nil then ld is nil
+if ld not nil then ed nil
+at least one is nil*)
+Proof with super_a.
+  intros.
+  generalize dependent SH_cont.
+  generalize dependent SH_ctup.
+  induction LH_cont_ld.
+  - intros.
+    exists sh_empty,SH_cont,
+      th_empty,SH_ctup...
+  - intros. inversion H...
+    apply IHLH_cont_ld in H4.
+    destruct H4 as
+      [SH_cont_ld' [SH_cont_ed' [SH_ctup_ld' [SH_ctup_ed' hyp]]]].
+    destruct hyp as
+      [hyp1 [hyp2 [hyp3 [hyp4 hyp5]]]].
+    exists
+      ((H_one_cont_ld ++ [(L_last,stack s_last)]) ++ SH_cont_ld'),
+      SH_cont_ed',
+      (L_rsp !->t tuple [loc_w (hloc L_last 4)];
+       SH_ctup_ld'),
+      SH_ctup_ed'.
+    repeat split;trysolve.
+    + econstructor...
+      apply tup_heap_nil_split in H7...
+    + super_a. rewrite app_assoc...
+    + extensionality x.
+      unfold th_update,th_comp.
+      destruct (h_eqb L_rsp x)...
+    + intros.
+      destruct (h_eqb L_rsp L) as []eqn:?.
+      * left...
+        apply tup_heap_nil_split in H7...
+        destruct L as [L].
+        inversion Heqb.
+        apply Nat.eqb_eq in H1...
+      * destruct hyp5 with (L:=L).
+        -- left...
+        -- right... unfold th_update.
+           rewrite Heqb...
+Qed.
+Lemma cont_heap_app :
+  forall C_mem LH_cont_ld LH_cont_ed
+         SH_cont_ld SH_cont_ed
+         SH_ctup_ld SH_ctup_ed,
+    (*L_last is label of last stack
+      in the Ks*)
+    LS_rel_cont_heap C_mem LH_cont_ld
+      (SH_cont_ld,SH_ctup_ld) ->
+    LS_rel_cont_heap C_mem LH_cont_ed
+      (SH_cont_ed,SH_ctup_ed) ->
+    (forall L,
+        SH_ctup_ed L = tuple []
+        \/ SH_ctup_ld L = tuple []) ->
+    LS_rel_cont_heap C_mem
+      (LH_cont_ld ++ LH_cont_ed)
+      (SH_cont_ld ++ SH_cont_ed,
+        th_comp SH_ctup_ld SH_ctup_ed).
+Proof with super_a.
+  intros.
+  generalize dependent SH_cont_ld.
+  generalize dependent SH_ctup_ld.
+  induction LH_cont_ld;
+    intros;inversion H...
+  apply IHLH_cont_ld in H6.
+  2:{ intros. specialize H1 with L.
+      destruct H1.
+      - left...
+      - right. unfold th_update in H1.
+        destruct (h_eqb L_rsp L)
+          as []eqn:?... }
+  rewrite <- app_assoc.
+  specialize H1 with (hloc_num L_rsp).
+  destruct H1.
+  - rewrite th_comp_comm_th_update...
+    econstructor...
+    unfold th_comp.
+    rewrite H9...
+  - unfold th_update in H1.
+    rewrite h_eqb_refl in H1...
+Qed.
+Lemma update_comp_cancel :
+  forall L lst H1 H2,
+    H1 L = tuple [] -> H2 L = tuple [] ->
+    (L !->t tuple []; th_comp H1 (L !->t tuple lst; H2))
+    = th_comp H1 H2.
+Proof with super_a.
+  intros. extensionality x.
+  unfold th_update,th_comp.
+  destruct L as [L],x as [x].
+  destruct (h_eqb L x) as []eqn:?...
+  unfold h_eqb in Heqb.
+  rewrite Nat.eqb_eq in Heqb...
+  rewrite H0,H...
+Qed.
+Lemma fresh_cont_lab_rel :
+  forall L LH_cont C_mem SH_cont SH_ctup,
+    fresh_cont_lab (obj_lab L) LH_cont = true ->
+    LS_rel_cont_heap C_mem
+      LH_cont (SH_cont,SH_ctup) ->
+    SH_ctup L = tuple [].
+Proof with super_a.
+  intros.
+  generalize dependent SH_ctup.
+  generalize dependent SH_cont.
+  induction LH_cont;intros;
+    inversion H0...
+  specialize IHLH_cont with
+    (SH_cont:=SH_cont0)
+    (SH_ctup:=SH_ctup0).
+  unfold th_update.
+  inversion H.
+  destruct (L_rsp =? L) as []eqn:?...
+  rewrite Heqb.
+  apply IHLH_cont...
+Qed.
