Lexa.v
@@ -1,25 +1,24 @@
 Require Import Lists.List. Import ListNotations.
 Require Import Strings.String.
 Require Import Program.Basics.
-From TLC Require Import LibLN.
-Declare Scope Lexi_scope.
-Open Scope Lexi_scope.
+Declare Scope Lexa_scope.
+Open Scope Lexa_scope.
 
 (* ------------ ------------ ------------
    ------------ ------------ ------------
    ----------- Abstract Syntax -----------
    ------------ ------------ ------------
    ------------ ------------ ------------ *)
+(* In the Coq formalization we represent variables
+   as de Brujin Indices.
 
-Inductive variable := 
-| dbjind_var : nat -> variable
-| free_var : var -> variable.
+   We also explicitly differentiate
+   between static constants and runtime generated constants,
+   since this makes the proof more natural to work with.*)
+Inductive dbj_index := dbj_ind : nat -> dbj_index.
 Inductive code_label := c_lab : string -> code_label.
 Inductive obj_label := obj_lab : nat -> obj_label.
 Inductive hdl_label := hdl_lab : nat -> hdl_label.
-(*Inductive data_label : Type := 
-| obj_data_lab : obj_label -> data_label
-| hdl_data_lab : hdl_label -> data_label.*)
 Inductive static_const : Type :=
 | nat_const : nat -> static_const
 | c_lab_const : code_label -> static_const.
@@ -30,12 +29,9 @@ Inductive runtime_const : Type :=
 | ns.
 Inductive value :=
 | const_val : static_const -> value
-| var_val : variable -> value.
+| ind_val : dbj_index -> value.
 Definition local_env : Type := list runtime_const.
-Inductive annotation : Type :=
-| tail
-| abort
-| general.
+Inductive annotation : Type := general.
 Inductive expr : Type :=
 | val_e : value -> expr
 | add : value -> value -> expr
@@ -54,8 +50,14 @@ with term : Type :=
 with a_frame: Type :=
   act_f : local_env -> term -> a_frame
 with h_frame : Type :=
-  handler_f : hdl_label -> obj_label ->
-              code_label -> annotation -> h_frame
+  hdl_f : hdl_label -> obj_label ->
+          code_label -> annotation -> h_frame
+(* In the paper, the evaluation context and continuation
+   are represented as list of frames that can be either 
+   activation frames or handler frames. In our Coq
+   formalization, we explicitly represent continuations
+   and evaluation contexts as list of handler led 
+   activation frames *)
 with hdl_led_frm_lst : Type :=
 | hdl_led_lst : h_frame -> list a_frame -> hdl_led_frm_lst
 with heap_cont : Type :=
@@ -64,17 +66,23 @@ with heap_cont : Type :=
 Inductive heap_tuple : Type :=
 | tuple : list runtime_const -> heap_tuple.
 Definition eval_context := list hdl_led_frm_lst.
+(* We also explicitly split the heap into heap of tuples
+   and heap of continuations *)
 Definition tup_heap := obj_label -> heap_tuple.
 Definition cont_heap := list (obj_label * heap_cont).
 Definition heap := (tup_heap * cont_heap)%type.
+(* Since code memory is represented as a meta language
+   function taking a code label and returning
+   a "function" in object language, ns_func is the
+   default return value which means that a code label
+   has no associated function *)
 Inductive function : Type :=
 | func : nat -> term -> function
 | ns_func.
 Definition code_mem : Type := code_label -> function.
 
 (* Coercions *)
-Coercion dbjind_var : nat >-> variable.
-Coercion free_var : var >-> variable.
+Coercion dbj_ind : nat >-> dbj_index.
 Coercion c_lab : string >-> code_label.
 Coercion nat_const : nat >-> static_const.
 Coercion c_lab_const : code_label >-> static_const.
@@ -84,17 +92,17 @@ Coercion hdl_lab_const : hdl_label >-> runtime_const.
 Coercion const_val : static_const >-> value.
 Coercion val_e : value >-> expr.
 
-(* ------------ ------------ ------------
-   ------------ ------------ ------------
-   ------------- Interpreter -------------
-   ------------ ------------ ------------
-   ------------ ------------ ------------ *)
+(* --------------------------------------
+   --------------------------------------
+   ------- Operational Semantics --------
+   --------------------------------------
+   -------------------------------------- *)
 
 (* --------------------------------------------
               Map Related Helpers
    -------------------------------------------- *)
 (* Heap *)
-Definition empty_tup := tuple nil.
+Definition empty_tup := tuple [].
 Definition h_eqb (a b : obj_label) := 
   match a,b with
   | obj_lab a', obj_lab b' => Nat.eqb a' b'
@@ -106,19 +114,19 @@ Definition th_update (m : tup_heap) (x : obj_label) (v : heap_tuple) :=
   fun x' => if h_eqb x x' then v else m x'.
 Notation "x '!->t' v ';' m" :=
   (th_update m x v)
-    (at level 100, v at next level, right associativity):Lexi_scope.
-Definition ch_update (m : cont_heap) (x : obj_label) (v : heap_cont) :=
+    (at level 100, v at next level, right associativity):Lexa_scope.
+Definition ch_update
+  (m : cont_heap) (x : obj_label) (v : heap_cont) :=
   (x,v) :: m.
 Notation "x '!->ch' v ';' m" :=
   (ch_update m x v)
-    (at level 100, v at next level, right associativity):Lexi_scope.
+    (at level 100, v at next level, right associativity):Lexa_scope.
 
 (* Environment *)
-Definition env_fetch (env: local_env) (var:variable)
+Definition env_fetch (env: local_env) (var:dbj_index)
   : runtime_const :=
   match var with
-  | dbjind_var n => nth n env ns
-  | free_var str => ns
+  | dbj_ind n => nth n env ns
   end.
 
 (* Code *)
@@ -136,31 +144,23 @@ Definition c_comp (c1:code_mem) (c2:code_mem) :=
            end.
 Notation "x '!->c' v ';' m" :=
   (c_update m x v)
-    (at level 100, v at next level, right associativity):Lexi_scope.
-(* annotation *)
-Definition a_eqb (a b : annotation) :=
-  match a,b with
-  | general,general => true
-  | tail,tail => true
-  | abort,abort => true
-  | _,_ => false
-  end.
+    (at level 100, v at next level, right associativity):Lexa_scope.
 (* --------------------------------------------
                   Other helpers
    -------------------------------------------- *)
 
 Fixpoint update_nth {A: Type} (n:nat) (lst:list A) (v:A) :=
   match n, lst with
-  | 0, cons x lst' => cons v lst'
-  | _, nil => nil
-  | S n', cons x lst' => update_nth n' lst' v
+  | 0, x :: lst' => v :: lst'
+  | _, [] => []
+  | S n', x :: lst' => update_nth n' lst' v
   end.
 
 (* E hat of paper *)
 Definition var_deref (E:local_env) (val:value)
   : runtime_const :=
   match val with
-  | var_val ind => env_fetch E ind
+  | ind_val ind => env_fetch E ind
   | const_val c => run_const c
   end.
 
@@ -174,8 +174,7 @@ Fixpoint fresh_cont_lab L (H_cont:cont_heap) :=
   end.
 Definition is_h_frm_general_hdl (f:h_frame) : bool :=
   match f with
-  | handler_f _ _ _ general => true
-  | _ => false
+  | hdl_f _ _ _ general => true
   end.
 (* --------------------------------------------
                Operational Semantics
@@ -203,14 +202,14 @@ Inductive step (C:code_mem) :
                  (L:obj_label) (lst:list runtime_const),
     var_deref E v = L -> tH L = tuple lst ->
     step C (tH,cH,K,E, bind (pi i v) t)
-      (tH,cH,K,(nth i lst ns) :: E,t) (* from (1+i) to i*)
+      (tH,cH,K,(nth i lst ns) :: E,t)
 | L_set : forall tH cH K E t (i:nat) (lst:list runtime_const)
                  (v v':value) (L:obj_label) (c:runtime_const),
     var_deref E v = L -> tH L = tuple lst ->
     i < List.length lst -> lst = [c] ->
     step C (tH,cH,K,E, bind (asgn v i v') t)
       (L !->t tuple (update_nth i lst (var_deref E v')); tH,
-         cH,K,(var_deref E v') :: E,t) (* from i-1 to i *)
+         cH,K,(var_deref E v') :: E,t)
 | L_app : forall H K E t t' (n:nat)
                  (v v':value) (lst:list value)
                  (lab:code_label) hf alst,
@@ -228,20 +227,18 @@ Inductive step (C:code_mem) :
          (v_env:value)
          (lab_body lab_op:code_label)
          (L:hdl_label) (L_env:obj_label),
-    (* L fresh *)
     var_deref E v_env = L_env ->
     C lab_body = func 2 t' ->
     step C (H,(hdl_led_lst hf alst) :: K,E, bind (handle lab_body lab_op general v_env) t)
-      (H,(hdl_led_lst (handler_f L L_env lab_op general) [])
+      (H,(hdl_led_lst (hdl_f L L_env lab_op general) [])
          :: (hdl_led_lst hf ((act_f E t)::alst)) :: K,
         [obj_lab_const L_env; hdl_lab_const L],t')
-(*L and L_env reversed because dbj index counts from inside *)
 | L_leave :
   forall H K E E' t alst hf
          (L:hdl_label) (L_env:obj_label)
          (lab_op:code_label) (v:value),
     step C (H,
-        (hdl_led_lst (handler_f L L_env lab_op general) [])
+        (hdl_led_lst (hdl_f L L_env lab_op general) [])
           :: (hdl_led_lst hf ((act_f E t)::alst)) :: K,
         E',val_term v)
       (H,(hdl_led_lst hf alst) :: K,(var_deref E' v) :: E,t)
@@ -255,11 +252,11 @@ Inductive step (C:code_mem) :
     C lab_op = func 3 t' ->
     fresh_cont_lab L_k LH_cont = true ->
     step C (LH_tup,LH_cont,
-        (hdl_led_lst (handler_f L L_env lab_op general) alst_to_cont) ::
+        (hdl_led_lst (hdl_f L L_env lab_op general) alst_to_cont) ::
           (hdl_led_lst hf alst) :: K,E,
         bind (raise general v1 v2) t)
       (LH_tup, L_k !->ch 
-                 cont [hdl_led_lst (handler_f L L_env lab_op general)
+                 cont [hdl_led_lst (hdl_f L L_env lab_op general)
                           ((act_f E t) :: alst_to_cont)];
        LH_cont,(hdl_led_lst hf alst) :: K,
          [obj_lab_const L_env;op_arg;obj_lab_const L_k],t')
@@ -274,14 +271,14 @@ Inductive step (C:code_mem) :
     fresh_cont_lab L_k LH_cont = true ->
     step C (LH_tup,LH_cont,
         hdl_led_lst hf_topmost alst_topmost :: K' ++
-          [hdl_led_lst (handler_f L L_env lab_op general) alst_to_cont] ++
-          hdl_led_lst (handler_f L_new L_envnew lab_opnew general) alst :: K,E,
+          [hdl_led_lst (hdl_f L L_env lab_op general) alst_to_cont] ++
+          hdl_led_lst (hdl_f L_new L_envnew lab_opnew general) alst :: K,E,
         bind (raise general v1 v2) t)
       (LH_tup, L_k !->ch 
                  cont (hdl_led_lst hf_topmost (act_f E t::alst_topmost) :: K' ++
-                         [hdl_led_lst (handler_f L L_env lab_op general) alst_to_cont]);
+                         [hdl_led_lst (hdl_f L L_env lab_op general) alst_to_cont]);
        LH_cont,(hdl_led_lst
-                  (handler_f L_new
+                  (hdl_f L_new
                      L_envnew lab_opnew general) alst) :: K,
          [obj_lab_const L_env;op_arg;obj_lab_const L_k],t')
 | L_resume_one_hdl :
@@ -318,12 +315,5 @@ Inductive step (C:code_mem) :
            [hdl_led_lst hf_cont alst_cont] ++
            hdl_led_lst hf (act_f E t :: alst) :: K,
          (var_deref E v2) :: E',t').
+Close Scope Lexa_scope.
 
-Close Scope Lexi_scope.
-
-(* Changes made:
-
-Lexi heap now also starts index from 0 rather than 1.
-
-Lexi's asignment/set ref/v[i]<-v' now has an assumption
-that i can't be out of range*)
