LexaToSalt.v
@@ -1,26 +1,27 @@
-From LSEH Require Import Lexi.
+From LSEH Require Import Lexa.
 Import Lists.List. Import ListNotations.
 Import Strings.String.
 From LSEH Require Import Salt.
-Module L := Lexi. Module S := Salt. 
+Module L := Lexa. Module S := Salt. 
 (* -------------- Helper Functions ----------------- *)
+(* The iota of APL, when only taking 1 argument *)
 Fixpoint iota i :=
   match i with
-  | S n => cons i (iota n)
-  | O => nil
+  | S n => i :: (iota n)
+  | O => []
   end.
 Fixpoint zip_map {A B C: Type} (func:A->B->C) lst1 lst2 :=
   match lst1,lst2 with
   | x1 :: lst1', x2 :: lst2' =>
     [func x1 x2] ++ (zip_map func lst1' lst2')
-  | _,_ => nil
+  | _,_ => []
   end.
 
 Fixpoint zip {A: Type} (lst1 lst2 : list A) :=
   match lst1,lst2 with
-  | cons x lst1', cons y lst2' => [x; y] ++ (zip lst1' lst2')
-  | nil, _ => lst2
-  | _, nil => lst1
+  | x :: lst1', y :: lst2' => [x; y] ++ (zip lst1' lst2')
+  | [], _ => lst2
+  | _, [] => lst1
   end.
 Definition r0 := nat_reg 0.
 Definition r1 := nat_reg 1.
@@ -29,16 +30,9 @@ Definition r3 := nat_reg 3.
 Definition r4 := nat_reg 4.
 Definition r5 := nat_reg 5.
 Definition r6 := nat_reg 6.
-(* -------- Translation for handler labels ------------ *)
-(* have a mapping storing what heap location in salt a
-   handler label maps to *)
-Definition handle_map := L.hdl_label -> S.heap_loc.
 
-(* -------------- Actual Translations ----------------- *)
 Definition annotation_trans (a:L.annotation) r : instr :=
   match a with
-  | L.tail => mov r 1
-  | L.abort => mov r 2
   | L.general => mov r 0
   end.
 Definition static_const_trans (c:L.static_const)
@@ -57,14 +51,13 @@ Definition run_cst_trans (v:L.runtime_const) : word :=
 Definition val_direct_trans (v:L.value)
   (stk_lst:list word) : S.word :=
   match v with
-  | L.var_val (dbjind_var n) =>
+  | L.ind_val (dbj_ind n) =>
     nth n stk_lst ns
-  | L.var_val (L.free_var _) => ns
   | L.const_val c => static_const_trans c
   end.
 Definition val_trans r (v:value) : instr :=
   match v with
-  | L.var_val (dbjind_var n) => load r sp false n
+  | L.ind_val (dbj_ind n) => load r sp false n
   | _ => mov r (val_direct_trans v [])
   end.
 
@@ -91,31 +84,21 @@ Definition expr_trans exp : list instr :=
     (L.c_lab clab_op) A v_env =>
     [annotation_trans A r4; val_trans r3 v_env;
       mov r2 (cloc clab_op 0); mov r1 (cloc clab_body 0);
-     call (if a_eqb L.general A
-           then cloc "handle"%string 0
-           else cloc "handle_same_stack"%string 0)]
+     call (cloc "handle"%string 0)]
   | L.raise L.general v1 v2 => [val_trans r2 v2; val_trans r1 v1;
     call (cloc "raise"%string 0)]
-  | L.raise L.tail v1 v2 => [val_trans r2 v2 ; val_trans r1 v1;
-    load r3 r1 false 3; load r1 r1 false 2 ; call r3]
   | L.resume v1 v2 => [val_trans r2 v2 ; val_trans r1 v1;
     call (cloc "resume"%string 0)]
-  (* Impossible case for newref continuation *)
-  | _ => []
   end.
 Fixpoint term_trans tm : list instr:=
   match tm with
   | L.val_term v => [val_trans r1 v]
-  | L.bind (L.raise L.abort v1 v2) t =>
-    [val_trans r2 v2 ; val_trans r1 v1;
-    load r3 r1 false 3; mov sp r1; load r1 r1 false 2;
-    sfree 4; jmp r3]        
   | L.bind exp t =>
     expr_trans exp
     ++ [push r1]
     ++ term_trans t
   (* special case, not needed for translating code,
-     but needed for relating lexi and salt's config *)
+     but needed for relating lexa and salt's config *)
   | L.halt => [S.halt]
   end.
 
@@ -145,9 +128,3 @@ Definition code_mem_trans (c:L.code_mem) : S.code_mem :=
   fun (x:code_loc) =>
   match x with cloc_str str => func_trans (c str) end.  
 
-(*
-All changes made
-0. register 1 and register 2 are swapped in addition and assignment
-1. in newref, malloc uses register r1 and values use r2, so that
-   we actually have L label on the stack, matching Lexi semantics
-*)
