SimProof.v
@@ -2,12 +2,12 @@ From LSEH Require Import Infrastructure.
 Import Lists.List. Import ListNotations.
 Import Strings.String.
 Import Logic.FunctionalExtensionality.
-Import RelConfig. Import LexiToSalt.
+Import RelConfig. Import LexaToSalt.
 Import PeanoNat. Import Lia.
-Import Lexi. Import Salt.
-Module L := Lexi. Module S := Salt. Module LS := LexiToSalt.
+Import Lexa. Import Salt.
+Module L := Lexa. Module S := Salt. Module LS := LexaToSalt.
 Module R := RelConfig.
-Delimit Scope Lexi_scope with L_scope.
+Delimit Scope Lexa_scope with L_scope.
 
 
 (* ----------------------------------------------------------
@@ -23,42 +23,11 @@ Inductive multi_plus {X : Type} (R : X -> X -> Prop) : X -> X -> Prop :=
 | multi_step : forall (x y z : X),
     R x y -> multi_plus R y z -> multi_plus R x z.
 (* -----------------------------------------------------------------
-    Theorem 2: translation from lexi to salt is semantic preserving
+    Theorem 2: translation from lexa to salt is semantic preserving
    ----------------------------------------------------------------- *)
 (* By Theorem 1 already proven, this is reduced to proving LS_rel satisfying
-  the 3 conditions *)
-Lemma one_eval_ctx_rel :
-  forall frm frm_lst C_mem L,
-    (LS_rel_hdl L frm frm_lst
-     /\ is_h_frm_general_hdl frm = true)
-    <->
-    LS_rel_eval_ctx C_mem [hdl_led_lst frm []]
-      [(hloc_str L,stack frm_lst)].
-Proof with super_a.
-  intros. split.
-  - intros.
-    apply rel_eval_ctx_lst with
-      (K:=hdl_led_lst frm [])...
-    apply rel_hdl_stk_base with
-      (Flst:=[]) (s:=[])...
-  - intros. split;
-      inversion H;subst;
-      inversion H5;subst;
-      inversion H7...
-    inversion H3...
-Qed.
-Lemma length_ctx_stk :
-  forall C_mem H K,
-    LS_rel_eval_ctx C_mem K H ->
-    List.length H <= List.length K.
-Proof with super_a.
-  intros C_mem H.
-  induction H...
-  intros. inversion H0;subst.
-  apply IHlist in H4.
-  apply le_n_S in H4.
-  rewrite H4. cbn...
-Qed.
+   the 3 conditions *)
+
 Theorem cond1 : forall C1 C2 M1 M2,
     code_mem_trans C1 = C2 -> init_L C1 M1 ->
     init_S C2 M2 -> LS_rel M1 M2.
@@ -91,7 +60,6 @@ Proof with super_a.
     + destruct (L.c_eqb init_lab x).
       * inversion Heqf... intros. destruct H2...
       * inversion Heqf...
-        (*- repeat apply_fresh lc_bind...*)
 Qed.
 
 Theorem cond2 : forall M1 M2 i,
@@ -103,1035 +71,7 @@ Proof with automate.
   apply nth_middle.
 Qed.
 
-Definition un_tuple (tup:tuple_heap_val) : list word :=
-  match tup with tuple lst => lst end.
-Definition un_stack stk : list word :=
-  match stk with
-  | stack lst => lst
-  end.
-Lemma tuple_un_tuple : forall h_val,
-    tuple (un_tuple h_val) = h_val.
-Proof with automate. intros. destruct h_val... Qed.
-Lemma stack_un_stack : forall lst,
-    stack (un_stack (stack lst)) = stack lst.
-Proof with automate. intros... Qed.
-Lemma term_trans_not_nil : forall tm,
-    term_trans tm <> [].
-Proof with automate.
-  intros. unfold not. destruct tm;simpl...
-  destruct e;intros;simpl;apply eq_sym in H;
-    generalize dependent H...
-  - apply app_cons_not_nil.
-  - destruct a...
-Qed.
-Lemma ins_verify : forall (A : Type) (l l' : list A) (d : A) (n : nat),
-    nth (n + List.length l) (l ++ l') d = nth n l' d.
-Proof.
-  intros. rewrite PeanoNat.Nat.add_comm.
-  apply app_nth2_plus.
-Qed.
-Lemma val_dir_trans_var_deref : forall E (v:value) lst,
-    (forall ind:nat, v = var_val ind -> ind < List.length E) ->
-    val_direct_trans v (List.map run_cst_trans E ++ lst)
-    = run_cst_trans (L.var_deref E v).
-Proof with super_a.
-  intros. destruct v as [|[|]]...
-  rewrite <- map_nth with (d:=L.ns)...
-  rewrite app_nth1... specialize H with n.
-  rewrite map_length...  
-Qed.
 
-Lemma stk_points_to_preserves :
-  forall s s' L' s_added,
-    3 < List.length s ->
-    stk_points_to s s' L' <->
-    stk_points_to (s_added ++ s) s' L'.
-Proof with super_a.
-  unfold stk_points_to.
-  intros. split;intros;
-    rewrite <- H0;
-    rewrite rev_app_distr with (y:=s);
-    rewrite nth_error_app1;super_a;
-    rewrite rev_length...    
-Qed.
-Definition get_hdl_lab (hdl_frm_lst:hdl_led_frm_lst) : nat :=
-  match hdl_frm_lst with
-  | hdl_led_lst (handler_f (hdl_lab L) _ _ _) _ => L
-  end.
-Definition frm_to_hloc frm :=
-  hloc_str (get_hdl_lab frm).
-Definition is_hdllst_general hdl_lst:=
-  match hdl_lst with
-  | hdl_led_lst frm alst =>
-      is_h_frm_general_hdl frm
-  end.
-Lemma last_eval_ctx_rel :
-  forall s L frm C_mem Ks H,
-    LS_rel_eval_ctx C_mem
-      (Ks ++ [frm])
-      (H ++ [(hloc_str L,stack s)]) ->
-    is_hdllst_general frm = true ->
-    LS_rel_hdl_stk C_mem L
-      frm (stack s)
-    /\ L = get_hdl_lab frm.
-Proof with super_a.
-  intros.
-  destruct frm as
-    [[[L_h] L_env lab_op []] alst];
-    trysolve.
-  generalize dependent H.
-  induction Ks.
-  - intros.
-    destruct H.
-    2:{ apply length_ctx_stk in H0.
-        rewrite app_length in H0.
-        rewrite Nat.add_comm in H0.
-        cbn in H0... }
-    inversion H0...
-    inversion H8...
-    inversion H5...
-  - intros. inversion H0;subst.
-    destruct H;inversion H5;
-      subst;trysolve.
-    inversion H6.
-    destruct Ks...
-Qed.
-Lemma eval_ctx_app_split :
-  forall C_mem K' K H,
-    LS_rel_eval_ctx C_mem
-      (K' ++ K) H ->
-    exists H_ld H_ed,
-      LS_rel_eval_ctx C_mem K' H_ld
-      /\ LS_rel_eval_ctx C_mem K H_ed
-      /\ H = H_ld ++ H_ed.
-Proof with super_a.
-  intros. generalize dependent H.
-  induction K'.
-  { intros.
-    exists sh_empty,H... }
-  intros. inversion H0...
-  apply IHK' in H4.
-  destruct H4 as
-    [H_ld [H_ed [hyp1 [hyp2 hyp3]]]].
-  exists ((hloc_str L,stack s)
-            :: H_ld),H_ed...
-  intros. eapply H7...
-Qed.
-Lemma eval_ctx_last_label :
-  forall C_mem H K' L frm,
-    LS_rel_eval_ctx C_mem
-      (K' ++ [frm]) H ->
-    is_hdllst_general frm = true ->
-    L = get_hdl_lab frm ->
-    exists H' s,
-      H = H' ++ [(hloc_str L,
-                   stack s)]
-      /\ 1 < List.length s.
-Proof with super_a.
-  intros.
-  destruct frm as
-    [[[L_h] L_env lab_op []] alst]...
-  generalize dependent H.
-  induction K'.
-  { intros. 
-    inversion H0...
-    exists sh_empty,s.
-    apply length_ctx_stk in H0.
-    inversion H5;inversion H6;
-    inversion H10...
-    rewrite app_length... }
-  intros. inversion H0...
-  apply IHK' in H5.
-  destruct H5 as [H' [s' [h1 h2]]].
-  exists ((hloc_str L, stack s) :: H'),s'...
-Qed.
-
-Lemma eval_ctx_app_comp :
-  forall C_mem K' K H_ld H_ed,
-    LS_rel_eval_ctx C_mem K' H_ld ->
-    LS_rel_eval_ctx C_mem K H_ed ->
-    (forall H_ld' H_ed' L s L' s',
-        H_ld = H_ld' ++ [(L,stack s)] ->
-        H_ed = (L',stack s') :: H_ed' ->
-        stk_points_to s s' L') ->
-    LS_rel_eval_ctx C_mem
-      (K' ++ K) (H_ld ++ H_ed).
-Proof with super_a.
-  intros. generalize dependent H_ld.
-  induction K'.
-  { intros. inversion H... }
-  destruct H_ed as [|b H_ed']eqn:?.
-  { intros. inversion H0...
-    repeat (rewrite app_nil_r)... }
-  intros. inversion H;subst.
-  pose proof H5 as H5_backup.
-  apply IHK' in H5.
-  { constructor...
-    intros.
-    destruct H2.
-    - (*destructing it means we prove the first of H_ed
-        is the s_pr ev of Hld*)
-      inversion H5_backup...
-      inversion H3...
-      specialize H1 with
-        (H_ld':=[]) (H_ed':=H')
-        (L:=hloc_str L) (s:=s).
-      assert (Tmp:[(L, stack s)] = [(L, stack s)])...
-    - inversion H3... }
-  (*also use H1 here *)
-  intros. inversion H4...
-  apply H1 with
-    (H_ld':=(hloc_str L,stack s)
-              :: H_ld')
-    (H_ed':=H_ed'0) (L:=L0)...
-Qed.
-(*Lemma eval_ctx_split_already :
-  forall C_mem K' K H_ld H_ed,
-    LS_rel_eval_ctx C_mem
-      (K' ++ K) (H_ld ++ H_ed) ->
-    LS_rel_eval_ctx C_mem K' H_ld
-    /\ LS_rel_eval_ctx C_mem K H_ed.
-Proof with super_a.
-  intros. generalize dependent H_ld.
-  induction K'.
-  { intros. split...
-Qed.
-Lemma eval_ctx_recompose :
-  forall C_mem K' K H_ld H_ed frm a,
-    LS_rel_eval_ctx C_mem K' H_ld ->
-    LS_rel_eval_ctx C_mem (frm :: K) (a :: H_ed) ->
-    LS_rel_eval_ctx C_mem
-      (K' ++ frm :: K) (H_ld ++ a :: H_ed) ->
-    LS_rel_eval_ctx C_mem (K' ++ [frm]) (H_ld ++ [a])
-    /\ LS_rel_eval_ctx C_mem K H_ed.
-Proof with super_a.
-  intros. split;inversion H0...
-  assert (K' ++ frm :: K
-          = K' ++ [frm] ++ K)...
-  rewrite H2 in H1.
-  assert (H_ld ++ (hloc_str L,stack s)
-            :: H_ed
-          = H_ld ++ [(hloc_str L,stack s)]
-              ++ H_ed)...
-  rewrite H3 in H1.
-  repeat (rewrite app_assoc in H1).
-  apply eval_ctx_app_split in H1.
-  destruct H1 as
-    [Hld [Hed [hyp1 [hyp2 hyp3]]]].
-  assert (Hed = H_ed).
-  { generalize dependent H_ed.
-    generalize dependent Hed.
-    induction K.
-    - intros.
-      inversion H7...
-      inversion hyp2...
-    - intros.
-      apply IHK...
-      + 
-      3:{
-      +
-      + inversion H7...
-      super_a.}
-  apply eval_ctx_last_label in hyp1.
-Qed.*)
-
-(*what I really need is just to prove that frm1 points
-to frm2, so that the s_prev and L_prev that we obtain
-is indeed what we have for frm2*)
-Lemma eval_ctx_app_2_middle :
-  forall C_mem K K' frm1 frm2 H,
-    LS_rel_eval_ctx C_mem
-      (K' ++ frm1 :: frm2 :: K) H ->
-    is_hdllst_general frm1 = true ->
-    is_hdllst_general frm2 = true ->
-    exists s1 s2 H_ld H_ed,
-      LS_rel_eval_ctx C_mem (K' ++ [frm1])
-        (H_ld ++ [(frm_to_hloc frm1,stack s1)])
-      /\ LS_rel_eval_ctx C_mem (frm2 :: K)
-           ((frm_to_hloc frm2,stack s2) :: H_ed)
-      /\ H = H_ld ++ (frm_to_hloc frm1,stack s1)
-               :: (frm_to_hloc frm2,stack s2) :: H_ed
-      /\ stk_points_to s1 s2 (frm_to_hloc frm2).
-Proof with super_a.
-  intros. generalize dependent H.
-  induction K'.
-  { intros. inversion H0...
-    inversion H6...
-    exists s,s0,sh_empty,H.
-    inversion H7;subst;
-    inversion H5;subst;
-    inversion H10;subst;
-    inversion H14... }
-  intros. inversion H0...
-  apply IHK' in H6.
-  destruct H6 as
-    [s1 [s2 [H_ld [H_ed hyp]]]].
-  destruct hyp as [hyp1 [hyp2 [hyp3 hyp4]]].
-  exists s1,s2,((hloc_str L,stack s)
-                  :: H_ld),H_ed...
-  intros. destruct H_ld;inversion H...
-  - eapply H9...
-  - eapply H9...
-Qed.
-Lemma app_inv_length_ld :
-  forall {A:Type} (l1 l2 l3 l4:list A),
-    l1 ++ l2 = l3 ++ l4 ->
-    List.length l2 = 5 ->
-    List.length l4 = 5->
-    l1 = l3.
-Proof with super_a.
-  intros.
-  assert (forall {A:Type} (l1 l2:list A),
-             l1 = l2 -> List.length l1
-                        = List.length l2)...
-  pose proof H as H3.
-  apply H2 in H3.
-  apply app_inv_tail with (l:=l2).
-  repeat (rewrite app_length in H3).
-  repeat (destruct l2 as [|];super_a).
-  repeat (destruct l4 as [|];super_a).
-  rewrite H. generalize dependent l1.
-  induction l3...
-  - destruct l1...
-  - intros. destruct l1.
-    + inversion H3...
-    + rewrite IHl3 with
-        (l1:=l1)...
-      inversion H...
-Qed.
-Lemma app_inv_length_ed :
-  forall {A:Type} (l1 l2 l3 l4:list A),
-    l1 ++ l2 = l3 ++ l4 ->
-    List.length l2 = 5 ->
-    List.length l4 = 5->
-    l2 = l4.
-Proof with super_a.
-  intros.
-  pose proof H.
-  apply app_inv_length_ld in H...
-  eapply app_inv_head...
-Qed.
-Lemma eval_ctx_last_points_to_preserves :
-  forall C_mem K H L s frmlst1 frmlst2 frm alst,
-    LS_rel_eval_ctx C_mem
-      (K ++ [hdl_led_lst frm alst])  
-      (H ++ [(hloc_str L, stack (s ++ frmlst1))]) ->
-    LS_rel_hdl L frm frmlst1 ->
-    LS_rel_hdl L frm frmlst2 ->
-    LS_rel_eval_ctx C_mem
-      (K ++ [hdl_led_lst frm alst])  
-      (H ++ [(hloc_str L, stack (s ++ frmlst2))]).
-Proof with super_a.
-  intros. inversion H1...
-  inversion H2...
-  generalize dependent K.
-  induction H...
-  - intros.
-    inversion H0...
-    inversion H8...
-    inversion H5...
-    + apply app_inv_length_ld
-        in H...
-    + inversion H5...
-      apply app_inv_length_ed
-        in H...
-  - intros.
-    destruct K;
-      inversion H0;subst.
-    { inversion H8.
-      destruct H... }
-    apply IHlist in H8.
-    constructor...
-    destruct H. 
-    + intros. 
-      inversion H...
-      unfold stk_points_to.
-      rewrite app_length.
-      assert (stk_points_to s0
-                (s ++
-                   [loc_w (cloc handle_loc 10);
-                    loc_w (hloc L_prev (Datatypes.length s_prev));
-                    int_w 0; 
-                    loc_w (hloc L_env 0);
-                    loc_w (cloc Clab_op 0)]) L).
-      { apply H10 with (H':=[])... }
-      unfold stk_points_to in H3.
-      rewrite app_length in H3...
-    + intros. inversion H3...
-      apply H10 with
-        (H':=H ++
-               [(hloc_str L,
-                  stack (s ++
-                           [loc_w (cloc handle_loc 10);
-                            loc_w (hloc L_prev (Datatypes.length s_prev));
-                            int_w 0; 
-                            loc_w (hloc L_env 0);
-                            loc_w (cloc Clab_op 0)]))])...
-Qed.
-
-Lemma app_inv_last :
-  forall {A:Type} (l1:list A) l2 a b,
-    l1 ++ [a] = l2 ++ [b] ->
-    a = b
-    /\ l1 = l2.
-Proof with super_a.
-  intros. generalize dependent l2.
-  induction l1.
-  - intros.
-    induction l2...
-    + inversion H...
-    + inversion H...
-      induction l2...
-    + induction l2...
-  - intros.
-    induction l2.
-    + induction l1...
-    + split.
-      * apply IHl1 with
-          (l2:=l2).
-        inversion H...
-      * inversion H...
-        apply IHl1 in H2.
-        destruct H2.
-        rewrite H1...
-Qed.
- (* intros.
-  apply eval_ctx_app_split in H0.
-  destruct H0 as
-    [H_ld [H_ed [hyp1 [hyp2 hyp3]]]].
-  
-  (* get s1 and H_ld *)
-  destruct frm1 as
-    [[[L] L_env lab_op A] alst].
-  destruct A...
-  pose proof hyp1 as hyp4.
-  apply eval_ctx_last_label in hyp4.
-  destruct hyp4 as
-    [H_ld' [s1 [hyp4 hyp5]]].
-  (* get s2 and H_ed *)
-  inversion hyp2...
-  exists s1,s,H_ld',H;
-    inversion H5;
-    inversion H6...
-  - rewrite <- app_assoc...
-  - apply eval_ctx_app_split in H0_backup.
-    destruct H0_backup as
-      [H_ld'' [H_ed'' [_ [hy1 hy2]]]]...
-    inversion hy1...
-    inversion H11...
-    (**88888888888888888888*)
-    assert (Tmp:K' ++ frm1 :: frm2 :: K
-                = (K' ++ [frm1]) ++ frm2 :: K).
-  { rewrite <- app_assoc... }
-  pose proof H0 as H0_backup.
-  rewrite Tmp in H0.
-  apply eval_ctx_app_split in H0.
-  destruct Tmp.
-  destruct H0 as
-    [H_ld [H_ed [hyp1 [hyp2 hyp3]]]].
-  (* get s1 and H_ld *)
-  destruct frm1 as
-    [[[L] L_env lab_op A] alst].
-  destruct A...
-  pose proof hyp1 as hyp4.
-  apply eval_ctx_last_label in hyp4.
-  destruct hyp4 as
-    [H_ld' [s1 [hyp4 hyp5]]].
-  (* get s2 and H_ed *)
-  inversion hyp2...
-  exists s1,s,H_ld',H;
-    inversion H5;
-    inversion H6...
-  - rewrite <- app_assoc...
-  - apply eval_ctx_app_split in H0_backup.
-    destruct H0_backup as
-      [H_ld'' [H_ed'' [_ [hy1 hy2]]]]...
-    inversion hy1...
-    assert (H0 = (L
-    inversion H11...
-    
-Qed.*)
-(*
-Lemma eval_ctx_app_middle :
-  forall C_mem K' K H L L_env lab_op alst,
-    LS_rel_eval_ctx C_mem
-      ((K' ++
-          [hdl_led_lst
-             (L.handler_f (L.hdl_lab L)
-                L_env lab_op L.general)
-             alst]) ++ K) H ->
-    exists s H_ld H_ed,
-      LS_rel_eval_ctx C_mem K'
-        (H_ld ++ [(hloc_str L,stack s)])
-      /\ LS_rel_eval_ctx C_mem K H_ed
-      /\ H = H_ld ++ [(hloc_str L,
-                        stack s)] ++ H_ed.
-Proof with super_a.
-  intros. apply eval_ctx_app_split in H0.
-  destruct H0 as
-    [H_ld [H_ed [h1 [h2 h3]]]]...
-    generalize dependent H.
-  induction K'.
-  { intros.
-    exists sh_empty,H... }
-  intros. inversion H0...
-  apply IHK' in H4.
-  destruct H4 as
-    [H_ld [H_ed [hyp1 [hyp2 hyp3]]]].
-  exists ((hloc_str L,stack s)
-            :: H_ld),H_ed...
-  intros. eapply H7...
-Qed.
-
-Lemma eval_ctx_app_middle :
-  forall C_mem hf_top hf alst_top alst_mid alst
-         K' K H L L_env lab_op,
-    LS_rel_eval_ctx C_mem
-      (K' ++
-         L.hdl_led_lst (L.handler_f (L.hdl_lab L)
-                          L_env lab_op L.general) alst_mid
-          :: K) H ->
-    exists s H_ld H_ed,
-      LS_rel_eval_ctx C_mem
-        (K' ++
-           [L.hdl_led_lst (L.handler_f (L.hdl_lab L)
-                             L_env lab_op L.general) alst_mid])
-        (H_ld ++ [(hloc_str L,stack s)])
-      /\ LS_rel_eval_ctx C_mem K H_ed
-      /\ H = H_ld ++ [(hloc_str L,stack s)] ++ H_ed.
-Proof with super_a.
-  intros. generalize dependent H.
-  induction K'.
-  { intros. inversion H0...
-    inversion H4...
-    assert (L1 = L).
-    { inversion H8...
-      inversion H11... }(*
-    inversion H... inversion H6...
-    inversion H2...*)
-    exists s0,[(hloc_str L0,stack s)],H.
-    split... intros. inversion H1... }
-  intros.
-  cbn in IHK'.
-  inversion H0...
-  inversion H4...
-  invresion H.
-  inversion H6...
-      inversion H2...
-      destruct H1...
-      { induction K1... }
-      apply IHK1 in H3.
-      destruct H3 as
-        [H_ld' [H_ed [hyp1 [hyp2 hyp3]]]].
-      esplit. exists H_ed.
-      (*exists
-        ((hloc_str L0,
-          stack
-            [loc_w (cloc handle_loc 10);
-             loc_w (hloc L_prev (Datatypes.length s_prev));
-             int_w 0; 
-             loc_w (hloc L_env0 0);
-             loc_w (cloc Clab_op 0)]) :: H_ld'),s,H_ed.*)
-      split...
-      * apply rel_eval_ctx_lst with
-          (K:=[h_f (handler_f (hdl_lab L0) (obj_lab L_env0) Clab_op general)])
-          (Ks:=K1 ++
-                 [L.h_f (L.handler_f (hdl_lab L) L_env lab_op L.general)])...
-        intros. apply H5 with (H':=H'++H_ed).
-        rewrite hyp3,H3...
-      * rewrite hyp3...
-Qed.
-Lemma eval_ctx_app_split :
-  forall C_mem H K1 K2 L L_env lab_op,
-    LS_rel_eval_ctx C_mem
-      (K1 ++ [L.h_f (L.handler_f (hdl_lab L) L_env lab_op L.general)]
-         ++ K2) H ->
-    exists H_ld H_ed,
-      LS_rel_eval_ctx C_mem
-        (K1 ++ [L.h_f (L.handler_f (hdl_lab L) L_env lab_op L.general)]) H_ld 
-      /\ LS_rel_eval_ctx C_mem K2 H_ed
-      /\ H = H_ld ++ H_ed.
-Proof with super_a.
-  intros. generalize dependent H.
-  induction K1.
-  { intros. inversion H0...
-    inversion H4...
-    inversion H... inversion H6...
-    inversion H2...
-    esplit. exists H1.
-    split...
-    apply rel_eval_ctx_lst with
-      (K:=[h_f (handler_f (hdl_lab L)
-                  (obj_lab L_env0) Clab_op general)])...
-    cbn... }
-  intros.
-  cbn in IHK1.
-  inversion H0...
-  inversion H4...
-  (* first chunk is
-     general hdl led frames *)
-  - inversion H...
-    (*first frame is general hdl
-      (activation frames empty)*)
-    + inversion H6...
-      inversion H2...
-      destruct H1...
-      { induction K1... }
-      apply IHK1 in H3.
-      destruct H3 as
-        [H_ld' [H_ed [hyp1 [hyp2 hyp3]]]].
-      esplit. exists H_ed.
-      (*exists
-        ((hloc_str L0,
-          stack
-            [loc_w (cloc handle_loc 10);
-             loc_w (hloc L_prev (Datatypes.length s_prev));
-             int_w 0; 
-             loc_w (hloc L_env0 0);
-             loc_w (cloc Clab_op 0)]) :: H_ld'),s,H_ed.*)
-      split...
-      * apply rel_eval_ctx_lst with
-          (K:=[h_f (handler_f (hdl_lab L0) (obj_lab L_env0) Clab_op general)])
-          (Ks:=K1 ++
-                 [L.h_f (L.handler_f (hdl_lab L) L_env lab_op L.general)])...
-        intros. apply H5 with (H':=H'++H_ed).
-        rewrite hyp3,H3...
-      * rewrite hyp3...
-    (*first frame is activation frame
-      (some activation frames following
-      the general handler) *)
-    + inversion H9... inversion H14...
-      inversion H2...
-      rewrite <- H15 in IHK1.
-      assert (LS_rel_eval_ctx C_mem ((Flst0 ++ [h_f frm]) ++ Ks)
-                ((hloc_str L0,stack (s' ++ frm_stk)) :: H1)).
-      { super_a. intros. apply H5 in H8.
-        rewrite <- app_assoc in H8.
-        apply stk_points_to_preserves
-          in H8...
-        inversion H6;rewrite app_length... }
-      apply IHK1 in H8.
-      destruct H8 as [H_ld' [H_ed [hyp1 [hyp2 hyp3]]]].
-      inversion hyp1...
-      { destruct K1... }
-      inversion hyp3...
-      esplit. exists H_ed.
-      (*inversion H17...
-        inversion H22...
-        exists
-          sh_empty,(loc_w (cloc C_lab (Datatypes.length lst))
-                      :: (run_cstlst_trans E) ++ s' ++ frm_stk),H_ed.
-        rewrite <- app_assoc. *)
-      rewrite <- app_assoc.
-      split...
-      * rewrite app_comm_cons.
-        apply rel_eval_ctx_lst with
-            (s:=loc_w (cloc C_lab (Datatypes.length lst))
-                  :: (run_cstlst_trans E) ++ s' ++ frm_stk)...          
-        -- inversion H18;
-              repeat (rewrite app_comm_cons);
-              rewrite app_assoc with (m:=s);
-              constructor...
-        -- intros. rewrite app_comm_cons.
-            rewrite <- stk_points_to_preserves...
-            inversion H6;rewrite app_length...
-      * cbn...
-Qed.
-(* prove that last pair's
-   label is indeed L,
-   when we split *)
-
-Lemma eval_ctx_last_label :
-  forall C_mem H K1 L L_env lab_op,
-    LS_rel_eval_ctx C_mem
-      (K1 ++ [L.h_f (L.handler_f (hdl_lab L) L_env
-                       lab_op L.general)]) H ->
-    exists H' s,
-      H = H' ++ [(hloc_str L,stack s)]
-      /\ 1 < List.length s.
-Proof with super_a.
-  intros. generalize dependent H.
-  induction K1.
-  { intros. exists sh_empty.
-    inversion H0...
-    apply length_ctx_stk in H0.
-    inversion H0...
-    destruct H1... exists s.
-    inversion H3...
-    - rewrite app_nil_r in H2...
-      inversion H4...
-      destruct Flst;inversion H...
-      inversion H1...
-      inversion H2...
-    - inversion H4...
-      rewrite app_length.
-      inversion H1... }
-  intros.
-  inversion H0...
-  inversion H4...
-  inversion H...
-  (* activation frames empty *)
-  - inversion H6...
-    inversion H2...
-    destruct H1...
-    { induction K1... }
-    apply IHK1 in H3.
-    destruct H3 as
-      [H' [s [hyp1 hyp2]]].
-    esplit. exists s.
-    rewrite hyp1,app_comm_cons...
-  (* some activation frames following
-     the general handler *)
-  - inversion H9... inversion H14...
-    inversion H2...
-    rewrite <- H15 in IHK1.
-    assert (LS_rel_eval_ctx C_mem ((Flst0 ++ [h_f frm]) ++ Ks)
-              ((hloc_str L0,stack (s' ++ frm_stk)) :: H1)).
-    { super_a. intros. apply H5 in H8.
-      rewrite <- app_assoc in H8.
-      apply stk_points_to_preserves
-        in H8...
-      inversion H6;rewrite app_length... }
-    apply IHK1 in H8.
-    destruct H8 as [H' [s [hyp1 hyp2]]].
-    destruct H'.
-    + destruct H1.
-      * exists sh_empty,
-          (loc_w (cloc C_lab (Datatypes.length lst))
-             :: (run_cstlst_trans E ++ s') ++ frm_stk).
-        split.
-        -- inversion hyp1...
-        -- cbn. rewrite app_length.
-           inversion H6...
-      * inversion hyp1...
-    + destruct H1.
-      * inversion hyp1...
-        induction H'...
-      * inversion hyp1...
-        exists
-          (((hloc_str L0,
-              stack (loc_w (cloc C_lab (Datatypes.length lst))
-                       :: (run_cstlst_trans E ++ s') ++ frm_stk)))
-             :: H'), s.
-        rewrite H17...
-Qed.
-Lemma eval_ctx_app_middle :
-  forall C_mem H K1 K2 L L_env lab_op,
-    LS_rel_eval_ctx C_mem
-      (K1 ++ [L.h_f (L.handler_f (hdl_lab L) L_env lab_op L.general)]
-         ++ K2) H ->
-    exists s H_ld H_ed,
-      LS_rel_eval_ctx C_mem
-        (K1 ++ [L.h_f (L.handler_f (hdl_lab L) L_env lab_op L.general)])
-        (H_ld ++ [(hloc_str L,stack s)])
-      /\ LS_rel_eval_ctx C_mem K2 H_ed
-      /\ H = H_ld ++ [(hloc_str L,stack s)] ++ H_ed.
-Proof with super_a.
-  intros.
-  apply eval_ctx_app_split in H0.
-  destruct H0 as
-    [H_ld' [H_ed [hyp1 [hyp2 hyp3]]]]...
-  pose proof hyp1 as hyp3.
-  apply eval_ctx_last_label in hyp1.
-  destruct hyp1 as [H' [s [hyp1 hyp4]]]...
-  rewrite <- app_assoc.
-  exists s,H',H_ed.
-  split...
-Qed.
-Check rel_env_context.
-Lemma env_ctx_app_middle :
-  forall C_mem (E:L.local_env) (K1 K2:L.eval_context) L L_env lab_op
-         H (sp_loc:string) (sp_s:list word),
-    LS_rel_env_context C_mem
-      (K1 ++ [L.h_f (L.handler_f (hdl_lab L)
-                       L_env lab_op L.general)] ++ K2,E)
-      (H,hloc sp_loc (List.length sp_s)) ->
-    exists s H_ld H_ed,
-      LS_rel_env_context C_mem
-        (K1 ++ [L.h_f (L.handler_f (hdl_lab L) L_env lab_op L.general)],E)
-        (H_ld ++ [(hloc_str L,stack s)],
-          hloc sp_loc (List.length sp_s))
-      /\ LS_rel_eval_ctx C_mem K2 H_ed
-      /\ H = H_ld ++ [(hloc_str L,stack s)] ++ H_ed
-      /\ (H_ld = [] -> L = sp_loc /\ s = sp_s).
-Proof with super_a.
-  intros. inversion H0...
-  apply eval_ctx_app_middle in H4.
-  destruct H4 as [s [H_ld [H_ed [hyp1 [hyp2 hyp3]]]]].
-Admitted.
-*)
-
-Lemma update_nth_one_iter :
-  forall {A} n a lst (v:A),
-    update_nth (S n) (a :: lst) v = a :: update_nth n lst v.
-Proof. intros. super_a. Qed.
-(*Lemma update_nth_one_off :
-  forall {A} n a lst (v:a),
-    update_nth (S n) (a :: lst) v = a :: update_nth n lst *)
-Lemma update_nth_split :
-  forall {A} l1 l2 n (v:A),
-    n <= Datatypes.length l2 ->
-    update_nth (List.length (l1 ++ l2) - n) (l1 ++ l2) v
-    = l1 ++ update_nth (List.length l2 - n) l2 v.
-Proof with super_a.
-  intros. induction l1;automate.
-  assert (List.length ((a :: l1) ++ l2)
-            = S (List.length (l1 ++ l2)));
-    automate. rewrite H0.
-  rewrite Nat.sub_succ_l.
-  2:{ rewrite app_length... }
-  rewrite <- app_comm_cons.
-  rewrite update_nth_one_iter...
-Qed.
-Lemma update_nth_length :
-  forall {A} n l (v:A),
-    List.length (update_nth n l v)
-    = List.length l.
-Proof with super_a.
-  intros. generalize dependent n.
-  induction l;destruct n...
-Qed.
-(*Lemma rel_frame_inv :
-   forall C_mem F s s',
-    LS_rel_frame C_mem F s -> LS_rel_frame C_mem F s' ->
-    s = s'.
-Proof with super_a.
-  intros.
-  (* expand s *)
-  inversion H...
-  inversion H4...
-  inversion H1...
-  (* expand s' *)
-  inversion H0...
-  inversion H12...
-  inversion H9...
-  rewrite H8 in H13.
-  rewrite H2 in H10
-  - intros. inversion H. inversion H0...
-  - intros. inversion H... inversion H0...
-    specialize IHF with (s:=s'0) (s':=s'1).
-    apply IHF in H5. inversion H3...
-    inversion H4...
-Qed.
-Lemma rel_frames_inv :
-  forall C_mem F s s',
-    LS_rel_frames C_mem F s -> LS_rel_frames C_mem F s' ->
-    s = s'.
-Proof with super_a.
-  intros C_mem F. induction F.
-  - intros. inversion H. inversion H0...
-  - intros. inversion H... inversion H0...
-    specialize IHF with (s:=s'0) (s':=s'1).
-    apply IHF in H5. inversion H3...
-    inversion H4...
-Qed.
-Lemma push1_before_tm : forall ft lst Ilst E t,
-          wf_func_tm ft ->
-          func_trans ft = ins_seq (lst ++ Ilst) ->
-          LS_rel_ins (E,t) (ins_seq (tl Ilst)) ->
-          nth 0 Ilst ns_ins = push (reg_o 1).
-Proof with super_a.
-  intros. 
-
-  Lemma update_nth_map: forall {A B:Type} ind (f:A->B) lst v,
-    update_nth ind (List.map f lst) (f v)
-    = (List.map f (L.update_nth ind lst v)).
-Proof with super_a.
-intros. Search (List.map _ _=_(List.map _ _)). Admitted.
-  Lemma Sn_n1 : forall n m, S n = n + 1.
-Proof. intros.  Qed.
-Lemma SSn_n2 : forall n, S (S n) = n + 2.*)
-
-(*what I need:
-split cont stacks of salt
-using knowledge of cont heap in lexa
-need to give base of cont and top of cont*)
-Lemma tup_heap_nil_split :
-  forall H1 H2 L,
-    th_comp H1 H2 L = tuple [] ->
-    H1 L = tuple [] /\ H2 L = tuple [].
-Proof with super_a.
-  intros. split;
-    unfold th_comp in H;
-    destruct (H1 L) as []eqn:?;
-                         destruct l...
-Qed.
-Lemma th_comp_comm_th_update :
-  forall x v H1 H2,
-    H2 x = tuple [] ->
-    th_comp (x !->t v; H1) H2 =
-      (x !->t v; th_comp H1 H2).
-Proof with super_a.
-  intros. extensionality x'.
-  unfold th_comp,th_update,
-    h_eqb. destruct x as [x],x' as [x'].
-  destruct (x =? x') as []eqn:?...
-  rewrite Nat.eqb_eq in Heqb.
-  destruct v as [[|]]...
-Qed.
-Lemma cont_heap_split :
-  forall C_mem LH_cont_ld LH_cont_ed
-         SH_cont SH_ctup,
-    (*L_last is label of last stack
-      in the Ks*)
-    LS_rel_cont_heap C_mem
-      (LH_cont_ld ++ LH_cont_ed)
-      (SH_cont,SH_ctup) ->
-    exists SH_cont_ld SH_cont_ed
-           SH_ctup_ld SH_ctup_ed,
-      LS_rel_cont_heap C_mem LH_cont_ld
-        (SH_cont_ld,SH_ctup_ld)
-      /\ LS_rel_cont_heap C_mem LH_cont_ed
-           (SH_cont_ed,SH_ctup_ed)
-      /\ SH_cont = SH_cont_ld ++ SH_cont_ed
-      /\ SH_ctup = th_comp SH_ctup_ld SH_ctup_ed
-      /\ (forall L,
-             SH_ctup_ed L = tuple []
-             \/ SH_ctup_ld L = tuple []).
-(*can't both be non nil.
-if ed not nil then ld is nil
-if ld not nil then ed nil
-at least one is nil*)
-Proof with super_a.
-  intros.
-  generalize dependent SH_cont.
-  generalize dependent SH_ctup.
-  induction LH_cont_ld.
-  - intros.
-    exists sh_empty,SH_cont,
-      th_empty,SH_ctup...
-  - intros. inversion H...
-    apply IHLH_cont_ld in H4.
-    destruct H4 as
-      [SH_cont_ld' [SH_cont_ed' [SH_ctup_ld' [SH_ctup_ed' hyp]]]].
-    destruct hyp as
-      [hyp1 [hyp2 [hyp3 [hyp4 hyp5]]]].
-    exists
-      ((H_one_cont_ld ++ [(L_last,stack s_last)]) ++ SH_cont_ld'),
-      SH_cont_ed',
-      (L_rsp !->t tuple [loc_w (hloc L_last 4)];
-       SH_ctup_ld'),
-      SH_ctup_ed'.
-    repeat split;trysolve.
-    + econstructor...
-      apply tup_heap_nil_split in H7...
-    + super_a. rewrite app_assoc...
-    + extensionality x.
-      unfold th_update,th_comp.
-      destruct (h_eqb L_rsp x)...
-    + intros.
-      destruct (h_eqb L_rsp L) as []eqn:?.
-      * left...
-        apply tup_heap_nil_split in H7...
-        destruct L as [L].
-        inversion Heqb.
-        apply Nat.eqb_eq in H1...
-      * destruct hyp5 with (L:=L).
-        -- left...
-        -- right... unfold th_update.
-           rewrite Heqb...
-Qed.
-Lemma cont_heap_app :
-  forall C_mem LH_cont_ld LH_cont_ed
-         SH_cont_ld SH_cont_ed
-         SH_ctup_ld SH_ctup_ed,
-    (*L_last is label of last stack
-      in the Ks*)
-    LS_rel_cont_heap C_mem LH_cont_ld
-      (SH_cont_ld,SH_ctup_ld) ->
-    LS_rel_cont_heap C_mem LH_cont_ed
-      (SH_cont_ed,SH_ctup_ed) ->
-    (forall L,
-        SH_ctup_ed L = tuple []
-        \/ SH_ctup_ld L = tuple []) ->
-    LS_rel_cont_heap C_mem
-      (LH_cont_ld ++ LH_cont_ed)
-      (SH_cont_ld ++ SH_cont_ed,
-        th_comp SH_ctup_ld SH_ctup_ed).
-Proof with super_a.
-  intros.
-  generalize dependent SH_cont_ld.
-  generalize dependent SH_ctup_ld.
-  induction LH_cont_ld;
-    intros;inversion H...
-  apply IHLH_cont_ld in H6.
-  2:{ intros. specialize H1 with L.
-      destruct H1.
-      - left...
-      - right. unfold th_update in H1.
-        destruct (h_eqb L_rsp L)
-          as []eqn:?... }
-  rewrite <- app_assoc.
-  specialize H1 with (hloc_str L_rsp).
-  destruct H1.
-  - rewrite th_comp_comm_th_update...
-    econstructor...
-    unfold th_comp.
-    rewrite H9...
-  - unfold th_update in H1.
-    rewrite h_eqb_refl in H1...
-Qed.
-Lemma update_comp_cancel :
-  forall L lst H1 H2,
-    H1 L = tuple [] -> H2 L = tuple [] ->
-    (L !->t tuple []; th_comp H1 (L !->t tuple lst; H2))
-    = th_comp H1 H2.
-Proof with super_a.
-  intros. extensionality x.
-  unfold th_update,th_comp.
-  destruct L as [L],x as [x].
-  destruct (h_eqb L x) as []eqn:?...
-  unfold h_eqb in Heqb.
-  rewrite Nat.eqb_eq in Heqb...
-  rewrite H0,H...
-Qed.
-Lemma fresh_cont_lab_rel :
-  forall L LH_cont C_mem SH_cont SH_ctup,
-    fresh_cont_lab (obj_lab L) LH_cont = true ->
-    LS_rel_cont_heap C_mem
-      LH_cont (SH_cont,SH_ctup) ->
-    SH_ctup L = tuple [].
-Proof with super_a.
-  intros.
-  generalize dependent SH_ctup.
-  generalize dependent SH_cont.
-  induction LH_cont;intros;
-    inversion H0...
-  specialize IHLH_cont with
-    (SH_cont:=SH_cont0)
-    (SH_ctup:=SH_ctup0).
-  unfold th_update.
-  inversion H.
-  destruct (L_rsp =? L) as []eqn:?...
-  rewrite Heqb.
-  apply IHLH_cont...
-Qed.
-(*Lemma cont_heap_split_middle :
-  forall C_mem LH_cont_ld LH_cont_ed
-         L_rsp Ks SH_cont SH_ctup,
-    (*L_last is label of last stack
-      in the Ks*)
-    LS_rel_cont_heap C_mem
-      (LH_cont_ld ++ (L_rsp, cont Ks) :: LH_cont_ed)
-      (SH_cont,SH_ctup) ->
-    exists SH_cont_ld SH_cont_ed
-           SH_one_cont_ld L_last
-           s_last,
-      LS_rel_cont_heap C_mem LH_cont_ld
-        (SH_cont_ld,SH_ctup_ld)
-      /\ LS_rel_cont_heap C_mem [cont Ks]
-           (SH_one_cont_ld ++ [(L_last,s_last)],
-             L_rsp !->t tuple [hloc L_last 4]; th_empty)
-      /\ LS_rel_cont_heap C_mem LH_cont_ed
-           (SH_cont_ed,SH_ctup_ed)
-      /\ SH_cont = SH_cont_ld ++
-                     SH_one_cont_ld ++ [(L_last,s_last)]
-                     ++ SH_cont_ed
-      /\ SH_ctup = (L_rsp !->t tuple [hloc L_last 4];
-                    th_comp SH_cont_ld SH_cont_ed).
-Proof with super_a.
-  
-Qed.*)
 Theorem cond3 : forall LC SC H1 K1 E1 t1 R2 H2 H1' K1' E1' t1',
     LS_rel (LC, H1, K1, E1, t1)
       (SC, H2, R2) ->
@@ -1239,7 +179,7 @@ Proof with super_a.
                (r0,o0);
                (r1,val_direct_trans v cur_stk_val);
                (r2,o2)] ++ R36)).
-      { destruct v as [cst|[ind|str]].
+      { destruct v as [cst|[ind]].
         - apply S_mov with (d:=r1)
                            (o:=val_direct_trans (const_val cst) cur_stk_val)
                            (R:=[(ip,loc_w l);
@@ -1258,14 +198,7 @@ Proof with super_a.
             (H_stk_ld:=[]).
           rewrite PeanoNat.Nat.sub_diag in Ins.
           eapply Ins...
-          inversion H10. rewrite H15... apply nth_middle.
-        - apply S_mov with
-            (d:=r1) (o:=val_direct_trans (var_val str) cur_stk_val)
-            (R:=[(ip,loc_w l);
-                 (sp,loc_w (hloc L_out (List.length cur_stk_val)));
-                 (r0,o0);(r1,o1);
-                 (r2,o2)] ++ R36)...
-          inversion H10... rewrite H15... apply nth_middle. }
+          inversion H10. rewrite H15... apply nth_middle. }
       constructor.
       apply S_push with
         (o:=r1)
@@ -1287,7 +220,7 @@ Proof with super_a.
         rewrite <- PeanoNat.Nat.add_succ_comm.
         apply rel_ins. inversion H2...
       * apply rel_env_context with (s_out:=s_out)...
-        destruct v as [cst|[ind|str]]...
+        destruct v as [cst|[ind]]...
         rewrite <- map_nth with (d:=L.ns). rewrite app_nth1...
         rewrite map_length.
         inversion H10... inversion H2...
@@ -1302,7 +235,7 @@ Proof with super_a.
     destruct L as [L_str].
     exists ((L_out,
               stack (loc_w (hloc L_str 0) :: cur_stk_val)) :: H_stks,
-             th_comp (hloc_str L_str !->t
+             th_comp (hloc_num L_str !->t
                         tuple ([val_direct_trans v cur_stk_val]); SH_tup)
              SH_ctup),
       ([(ip,loc_w (incr_cloc 4 l));
@@ -1314,7 +247,7 @@ Proof with super_a.
     (* stepping salt code for newref *)
     + apply multi_step with
         (y:=((cur_stkh,
-               th_comp (hloc_str L_str !->t
+               th_comp (hloc_num L_str !->t
                  tuple ([ns]);SH_tup) SH_ctup),
               [(ip,loc_w (next_cloc l));
                (sp,loc_w (hloc L_out (List.length cur_stk_val)));
@@ -1330,7 +263,7 @@ Proof with super_a.
         - rewrite H15. inversion H10... apply nth_middle. }
       apply multi_step with
         (y:=((cur_stkh,
-               th_comp (hloc_str L_str !->t
+               th_comp (hloc_num L_str !->t
                           tuple ([ns]);SH_tup) SH_ctup),
               [(ip,loc_w (incr_cloc 2 l));
                (sp,loc_w (hloc L_out (List.length cur_stk_val)));
@@ -1338,7 +271,7 @@ Proof with super_a.
                (r1,loc_w (hloc L_str 0));
                (r2,val_direct_trans v cur_stk_val)]
                 ++ R36)).
-      { destruct v as [cst|[ind|str]].
+      { destruct v as [cst|[ind]].
         - apply S_mov with
             (d:=r2) (o:=val_direct_trans (const_val cst) cur_stk_val)
             (R:=[(ip,loc_w (next_cloc l));
@@ -1359,18 +292,10 @@ Proof with super_a.
                  (r2,o2)] ++ R36) (H_stk_ld:=[]).
           rewrite PeanoNat.Nat.sub_diag in Ins.
           eapply Ins...
-          + inversion H10. rewrite H15... apply ins_verify with (n:=1).
-        - apply S_mov with
-            (d:=r2) (o:=val_direct_trans (var_val str) cur_stk_val)
-            (R:=[(ip,loc_w (next_cloc l));
-                 (sp,loc_w (hloc L_out (List.length cur_stk_val)));
-                 (r0,o0);
-                 (r1,loc_w (hloc L_str 0));
-                 (r2,o2)] ++ R36)...
-          rewrite H15. inversion H10... apply ins_verify with (n:=1). }
+          + inversion H10. rewrite H15... apply ins_verify with (n:=1). }
       apply multi_step with
         (y:=((cur_stkh,
-               th_comp (hloc_str L_str !->t
+               th_comp (hloc_num L_str !->t
                  tuple ([val_direct_trans v cur_stk_val]);SH_tup) SH_ctup),
               [(ip,loc_w (incr_cloc 3 l));
                (sp,loc_w (hloc L_out (List.length cur_stk_val)));
@@ -1379,8 +304,8 @@ Proof with super_a.
                (r2,val_direct_trans v cur_stk_val)]
                 ++ R36)).
       { pose proof S_store_v as Ins. specialize Ins with
-          (d:=r1) (o:=reg_o r2) (j:=0) (L:=hloc_str L_str)
-          (H_vtup:=hloc_str L_str !->t
+          (d:=r1) (o:=reg_o r2) (j:=0) (L:=hloc_num L_str)
+          (H_vtup:=hloc_num L_str !->t
                  tuple ([ns]);SH_tup) (lst:=[ns])
           (R:=[(ip,loc_w (incr_cloc 2 l));
                (sp,loc_w (hloc L_out (List.length cur_stk_val)));
@@ -1413,12 +338,12 @@ Proof with super_a.
       * apply rel_env_context with (s_out:=s_out)...
       * unfold th_update,L.th_update,L.h_eqb,h_eqb.
         intros. destruct (Nat.eqb L_str L_tup)...
-        -- inversion H1... destruct v as [|[|]]...
+        -- inversion H1... destruct v as [|[]]...
            rewrite <- map_nth with (d:=L.ns)...
            rewrite app_nth1... inversion H2...
            inversion H16...
-           specialize H6 with (v:=L.var_val n).
-           assert (Temp:In (L.var_val n) [L.var_val (L.dbjind_var n)]).
+           specialize H6 with (v:=L.ind_val n).
+           assert (Temp:In (L.ind_val n) [L.ind_val (L.dbj_ind n)]).
            { super_a. } apply H6 in Temp. inversion Temp...
            rewrite List.map_length...
         -- inversion H7...
@@ -1447,7 +372,7 @@ Proof with super_a.
                (r0,o0);
                (r1,val_direct_trans v cur_stk_val);
                (r2,o2)] ++ R36)).
-      { destruct v as [cst|[ind|str]].
+      { destruct v as [cst|[ind]].
         - apply S_mov with
             (d:=r1) (o:=val_direct_trans (const_val cst) cur_stk_val) (l:=l)
             (R:=[(ip,loc_w l);(sp,loc_w (hloc L_out (List.length cur_stk_val)));
@@ -1462,12 +387,7 @@ Proof with super_a.
                  (r2,o2)] ++ R36) (H_stk_ld:=[]).
           rewrite PeanoNat.Nat.sub_diag in Ins. 
           eapply Ins...
-          inversion H10. rewrite H15... apply nth_middle.
-        - apply S_mov with
-            (d:=r1) (o:=val_direct_trans (var_val str) cur_stk_val)
-            (R:=[(ip,loc_w l);(sp,loc_w (hloc L_out (List.length cur_stk_val)));
-                 (r0,o0);(r1,o1);
-                 (r2,o2)] ++ R36)... }
+          inversion H10. rewrite H15... apply nth_middle. }
       apply multi_step with
         (y:=((cur_stkh,SH_tups),
               [(ip,loc_w (incr_cloc 2 l));
@@ -1484,7 +404,7 @@ Proof with super_a.
                (r2,o2)] ++ R36)...
         - rewrite H15. inversion H10...
           apply ins_verify with (n:=1).
-        - destruct v as [cst|[ind|str]]...
+        - destruct v as [cst|[ind]]...
           inversion H4... rewrite app_nth1.
           rewrite map_nth with (d:=L.ns).
           rewrite H2... rewrite map_length.
@@ -1520,7 +440,7 @@ Proof with super_a.
     exists ((L_out,
               stack (val_direct_trans v' cur_stk_val :: cur_stk_val))
               :: H_stks,
-             th_comp (hloc_str L_str !->t
+             th_comp (hloc_num L_str !->t
                         tuple (update_nth 0 (List.map run_cst_trans [c])
                                  (val_direct_trans v' cur_stk_val)); SH_tup) SH_ctup),
       ([(ip,loc_w (incr_cloc 4 l));
@@ -1536,7 +456,7 @@ Proof with super_a.
                (r0,o0);
                (r1,val_direct_trans v' cur_stk_val);
                (r2,o2)] ++ R36)).
-      { destruct v' as [cst|[ind|str]].
+      { destruct v' as [cst|[ind]].
         - apply S_mov with
             (d:=r1) (o:=val_direct_trans (const_val cst) cur_stk_val)
             (R:=[(ip,loc_w l);(sp,loc_w (hloc L_out (List.length cur_stk_val)));
@@ -1552,13 +472,7 @@ Proof with super_a.
                  (r2,o2)] ++ R36) (H_stk_ld:=[]).
           rewrite PeanoNat.Nat.sub_diag in Ins.
           eapply Ins...
-          + inversion H10. rewrite H15... apply nth_middle.
-        - apply S_mov with
-            (d:=r1) (o:=val_direct_trans (var_val str) cur_stk_val)
-            (R:=[(ip,loc_w l);(sp,loc_w (hloc L_out (List.length cur_stk_val)));
-                 (r0,o0);(r1,o1);
-                 (r2,o2)] ++ R36)...
-          rewrite H15. inversion H10... apply nth_middle. }
+          + inversion H10. rewrite H15... apply nth_middle. }
       apply multi_step with
         (y:=((cur_stkh,SH_tups),
               [(ip,loc_w (incr_cloc 2 l));
@@ -1566,7 +480,7 @@ Proof with super_a.
                (r0,o0);
                (r1,val_direct_trans v' cur_stk_val);
                (r2,loc_w (hloc L_str 0))] ++ R36)).
-      { destruct v as [cst|[ind|str]].
+      { destruct v as [cst|[ind]].
         - apply S_mov with
             (d:=r2) (o:=loc_w (hloc L_str 0))
             (R:=[(ip,loc_w (next_cloc l));(sp,loc_w (hloc L_out (List.length cur_stk_val)));
@@ -1592,11 +506,10 @@ Proof with super_a.
             inversion H10... inversion H3...
             inversion H7... inversion H6... }
           rewrite Temp. eapply Ins...
-          + inversion H10. rewrite H15... apply ins_verify with (n:=1).
-        - inversion H5... }
+          + inversion H10. rewrite H15... apply ins_verify with (n:=1). }
       apply multi_step with
         (y:=((cur_stkh,
-               th_comp (hloc_str L_str !->t
+               th_comp (hloc_num L_str !->t
                           tuple (update_nth 0 (List.map run_cst_trans [c])
                                    (val_direct_trans v' cur_stk_val));
                         SH_tup) SH_ctup),
@@ -1606,7 +519,7 @@ Proof with super_a.
                (r1,val_direct_trans v' cur_stk_val);
                (r2,loc_w (hloc L_str 0))] ++ R36)).
       { apply S_store_v with
-          (d:=r2) (o:=r1) (j:=0) (L:=hloc_str L_str)
+          (d:=r2) (o:=r1) (j:=0) (L:=hloc_num L_str)
           (lst:=List.map run_cst_trans [c])
           (R:=[(ip,loc_w (incr_cloc 2 l));
                (sp,loc_w (hloc L_out (List.length cur_stk_val)));
@@ -1637,7 +550,7 @@ Proof with super_a.
         rewrite <- Heql. rewrite <- PeanoNat.Nat.add_succ_comm.
         apply rel_ins. inversion H2...
       * apply rel_env_context with (s_out:=s_out)...
-        destruct v'... destruct v0...
+        destruct v' as [|[]]...
         rewrite <- map_nth with (d:=L.ns).
         rewrite app_nth1... rewrite map_length.
         inversion H2... inversion H6...
@@ -1645,7 +558,7 @@ Proof with super_a.
       * unfold th_update,L.th_update,L.h_eqb,h_eqb.
         inversion H18...
         intros. destruct (Nat.eqb L_str L_tup)...
-        -- inversion H1... destruct v' as [|[|]]...
+        -- inversion H1... destruct v' as [|[]]...
            rewrite <- map_nth with (d:=L.ns)...
            rewrite app_nth1... inversion H2... inversion H7...
            rewrite List.map_length.
@@ -1675,7 +588,7 @@ Proof with super_a.
                (sp,loc_w (hloc L_out (List.length cur_stk_val)));
                (r0,loc_w (cloc lab 0));
                (r1,o1);(r2,o2)] ++ R36)).
-      { destruct v as [cst|[ind|str]].
+      { destruct v as [cst|[ind]].
         - apply S_mov with
             (d:=r0) (o:=loc_w (cloc lab 0))
             (R:=[(ip,loc_w l);
@@ -1701,8 +614,7 @@ Proof with super_a.
             inversion H10... inversion H3... inversion H8...
             inversion H11... }
           rewrite Temp. eapply Ins...
-          + inversion H10. rewrite H15... apply nth_middle.
-        - inversion H7... }
+          + inversion H10. rewrite H15... apply nth_middle. }
       apply multi_step with
         (y:=(cur_stkh,SH_tups,
               [(ip,loc_w (incr_cloc 2 l));
@@ -1710,7 +622,7 @@ Proof with super_a.
                (r0,loc_w (cloc lab 0));
                (r1,val_direct_trans v' cur_stk_val);
                (r2,o2)] ++ R36)).
-      { destruct v' as [cst|[ind|str]].
+      { destruct v' as [cst|[ind]].
         - apply S_mov with
             (d:=r1) (o:=val_direct_trans (const_val cst) cur_stk_val)
             (R:=[(ip,loc_w (next_cloc l));
@@ -1729,15 +641,7 @@ Proof with super_a.
                  (r1,o1);(r2,o2)] ++ R36) (H_stk_ld:=[]).
           rewrite PeanoNat.Nat.sub_diag in Ins.
           eapply Ins...
-          + inversion H10. rewrite H15... apply ins_verify with (n:=1).
-        - apply S_mov with
-            (d:=r1) (o:=val_direct_trans (var_val str) cur_stk_val)
-            (R:=[(ip,loc_w (next_cloc l));
-                 (sp,loc_w (hloc L_out (List.length cur_stk_val)));
-                 (r0,loc_w (cloc lab 0));
-                 (r1,o1);(r2,o2)] ++ R36)...
-          rewrite H15. inversion H10... inversion H7...
-          apply ins_verify with (n:=1). }
+          + inversion H10. rewrite H15... apply ins_verify with (n:=1). }
       apply multi_step with
         (y:=((L_out, stack (loc_w (incr_cloc 3 l) :: cur_stk_val)) :: H_stks,
               SH_tups,
@@ -1799,12 +703,12 @@ Proof with super_a.
             apply stk_points_to_preserves...
             inversion H16... inversion H11...
             rewrite app_length... }
-        destruct v' as [cst|[ind|str]]...
+        destruct v' as [cst|[ind]]...
         rewrite <- map_nth with (d:=L.ns). rewrite app_nth1...
         inversion H2... rewrite List.map_length.
         inversion H6...
-        specialize H4 with (v':=L.var_val ind).
-        assert (Temp:In (L.var_val ind) [L.var_val (L.dbjind_var ind)]).
+        specialize H4 with (v':=L.ind_val ind).
+        assert (Temp:In (L.ind_val ind) [L.ind_val (L.dbj_ind ind)]).
         { super_a. } apply H4 in Temp. inversion Temp...
       * inversion H14... inversion H18.
         apply H4 in H6. unfold c_comp.
@@ -1832,7 +736,7 @@ Proof with super_a.
              (r0,o0);
              (r1,val_direct_trans v cur_stk_val);
              (r2,o2)] ++ R36)).
-    { destruct v as [cst|[ind|str]].
+    { destruct v as [cst|[ind]].
       - apply S_mov with
           (d:=r1) (o:=val_direct_trans (const_val cst) cur_stk_val)
           (R:=[(ip,loc_w l);
@@ -1850,14 +754,7 @@ Proof with super_a.
                (r2,o2)] ++ R36) (H_stk_ld:=[]).
         rewrite PeanoNat.Nat.sub_diag in Ins.
         eapply Ins...
-        + inversion H10. rewrite H15... apply nth_middle.
-      - apply S_mov with
-          (d:=r1) (o:=val_direct_trans (var_val str) cur_stk_val)
-          (R:=[(ip,loc_w l);
-               (sp,loc_w (hloc L_out (List.length cur_stk_val)));
-               (r0,o0);(r1,o1);
-               (r2,o2)] ++ R36)...
-        inversion H10... rewrite H15... apply nth_middle. }
+        + inversion H10. rewrite H15... apply nth_middle. }
     apply multi_step with
       (y:=((L_out,stack s_out) :: H_stks,SH_tups,
             [(ip,loc_w (incr_cloc 2 l));
@@ -1881,7 +778,7 @@ Proof with super_a.
       rewrite Temp in Hyp. rewrite <- Temp2.
       apply Hyp...
       - rewrite H15. inversion H10...
-        destruct v as [cst|[ind|str]];
+        destruct v as [cst|[ind]];
           rewrite PeanoNat.Nat.add_comm;
           apply ins_verify with (n:=1).
       - rewrite app_length, PeanoNat.Nat.add_comm.
@@ -1893,58 +790,9 @@ Proof with super_a.
         inversion H6. induction s... }
       eapply S_ret...
       - rewrite H15. inversion H10...
-        destruct v as [|[|]];
+        destruct v as [|[]];
           apply ins_verify with (n:=2).
       - induction s_out... }
-     
-    (* apply multi_step with
-      (y:=((L_out,stack (tl s_out)) :: H_stks,SH_tups,
-            [(ip,hd ns s_out);
-             (sp,loc_w (hloc L_out (List.length (tl s_out))));
-             (r0,o0);
-             (r1,val_direct_trans v cur_stk_val);
-             (r2,o2)] ++ R36)).
-    
-    { inversion H5;subst.
-      pose proof S_ret as Hyp. specialize Hyp with
-        (l:=cloc Clab (2 + (List.length lst))).
-      remember (fun (s_prev:list word) (lst0:list instr) C_lab =>
-                   [(ip,loc_w (cloc Clab (2 + (List.length lst))));
-                    (sp,loc_w (hloc L_out (S (List.length s_prev))));
-                    (r0,o0);
-                    (r1,
-                      val_direct_trans v
-                        (List.map run_cst_trans E1 ++
-                           loc_w (cloc C_lab (List.length lst0)) :: s_prev));
-                    (r2,o2);(r3,o3);
-                    (r4,o4);(r5,o5);(r6,o6)])
-        as newR.
-      revert HeqnewR.
-      inversion H8... 
-      - inversion H1... inversion H11...
-        remember ((s ++ s') ++ frm_stk) as s_prev.
-        intros.
-        specialize Hyp with
-          (pred_j:=List.length s_prev)
-          (*l':=cloc C_lab (List.length lst0)*)
-          (lst:=loc_w (cloc C_lab (Datatypes.length lst0))
-                  :: (s ++ s') ++ frm_stk)
-          (R:=newR s_prev lst0 C_lab)...
-        cbn in Hyp. apply Hyp...
-        rewrite H15. inversion H10...
-        destruct v as [|[|]];rewrite PeanoNat.Nat.add_comm;
-          apply ins_verify with (n:=2).
-      - inversion H3... inversion H16...
-        remember ((s ++ s') ++ frm_stk ++ slst) as s_prev.
-        intros.
-        specialize Hyp with
-          (pred_j:=List.length s_prev)
-          (lst:=loc_w (cloc C_lab (List.length lst0)) :: s_prev)
-          (R:=newR s_prev lst0 C_lab)...
-        cbn in Hyp. apply Hyp...
-        rewrite H15. inversion H10...
-        destruct v as [|[|]];rewrite PeanoNat.Nat.add_comm;
-          apply ins_verify with (n:=2). }*)
     constructor.
     { revert Heqcur_stk_val.
       revert HeqR36.
@@ -1984,7 +832,7 @@ Proof with super_a.
             rewrite app_length. inversion H6... 
           + rewrite app_assoc.
             inversion H20...
-            destruct v as [cst|[ind|str]]...
+            destruct v as [cst|[ind]]...
             rewrite <- map_nth with (d:=L.ns).
             rewrite app_nth1... inversion H10...
             rewrite List.map_length.
@@ -1994,32 +842,14 @@ Proof with super_a.
   - (* handle P_body with A P_op under v_env in t*)
     destruct lab_op as [lab_op],
         lab_body as [lab_body], L as [L].
-    (*exists
-      ((hloc_str L,
-         stack
-           [val_direct_trans v_env cur_stk_val;
-            loc_w (hloc L 4);loc_w (cloc handle_loc 10);
-            loc_w (hloc L_out (S (List.length cur_stk_val)));
-            int_w 0;
-            val_direct_trans v_env cur_stk_val; 
-            loc_w (cloc (cloc_str lab_op) 0)])
-         :: (L_out, stack (loc_w (incr_cloc 5 l) :: cur_stk_val))
-         :: H_stks, SH_tups, SH_conts),
-      ([(ip,loc_w (cloc lab_body 2));
-        (sp,loc_w (hloc L 7));(r0, o0);
-        (r1,val_direct_trans v_env cur_stk_val);
-        (r2,loc_w (hloc L 4));
-        (r3,val_direct_trans v_env cur_stk_val);
-        (r4,int_w 0);
-        (r5,loc_w (hloc L_out (S (List.length cur_stk_val))));
-        (r6,loc_w (cloc lab_body 0))]).*) esplit. esplit.
+    esplit. esplit.
     split.
     + rewrite HeqR36. eapply multi_step.
       { eapply S_mov with (d:=r4) (o:=0)...
         inversion H10... rewrite H15...
         apply nth_middle. }
       eapply multi_step.
-      { destruct v_env as [|[|]].
+      { destruct v_env as [|[]].
         - eapply S_mov with
             (d:=r3) (o:=val_direct_trans s cur_stk_val)...
         - pose proof S_load_stk as Temp.
@@ -2030,9 +860,7 @@ Proof with super_a.
           rewrite PeanoNat.Nat.sub_diag in Temp.
           eapply Temp...
           + rewrite H15. inversion H10...
-            apply ins_verify with (n:=1).
-        - eapply S_mov with
-            (d:=r3) (o:=val_direct_trans (var_val v) cur_stk_val)... }
+            apply ins_verify with (n:=1). }
       eapply multi_step.
       { eapply S_mov with
           (d:=r2) (o:=wd_o (cloc lab_op 0))...
@@ -2117,7 +945,7 @@ Proof with super_a.
                - rewrite H15,
                    <- app_assoc...
                - rewrite app_length... }
-        -- destruct v_env as [|[|]],L_env...
+        -- destruct v_env as [|[]],L_env...
            rewrite app_nth1. rewrite map_nth with (d:=L.ns).
            inversion H6... rewrite H2...
            apply rel_hdl_stk_base with
@@ -2128,7 +956,7 @@ Proof with super_a.
            inversion H10... inversion H2...
            inversion H7... inversion H3...
         -- intros. inversion H1...
-        -- destruct v_env as [|[|]],L_env...
+        -- destruct v_env as [|[]],L_env...
            rewrite app_nth1. rewrite map_nth with (d:=L.ns).
            inversion H6... rewrite H2...
            rewrite map_length.
@@ -2147,9 +975,9 @@ Proof with super_a.
     inversion H7...
     inversion H6...
     specialize H11 with
-      (L':=hloc_str L1) (s':=s) (H':=H1).
-    assert (Temp:(hloc_str L1, stack s) :: H1
-                 = (hloc_str L1, stack s) :: H1)...
+      (L':=hloc_num L1) (s':=s) (H':=H1).
+    assert (Temp:(hloc_num L1, stack s) :: H1
+                 = (hloc_num L1, stack s) :: H1)...
     apply H11 in Temp.
     unfold stk_points_to in Temp.
     inversion Temp...
@@ -2169,7 +997,7 @@ Proof with super_a.
         as cur_stk_val.
     esplit. esplit. split.
     + eapply multi_step.
-      { destruct v as [cst|[ind|var]].
+      { destruct v as [cst|[ind]].
         - eapply S_mov with
             (d:=r1) (o:=val_direct_trans cst cur_stk_val)...
           cbn. rewrite H15. inversion H10... apply nth_middle.
@@ -2178,20 +1006,17 @@ Proof with super_a.
           specialize Temp with
             (d:=r1) (load_off:=ind) (lst:=cur_stk_val)
             (reg_off:=List.length cur_stk_val) (s:=sp)
-            (H_stk_ld:=[]) (L:=hloc_str L0)
-            (H_stk_ed:=(hloc_str L1, stack s) :: H1 ++ SH_cont).
+            (H_stk_ld:=[]) (L:=hloc_num L0)
+            (H_stk_ed:=(hloc_num L1, stack s) :: H1 ++ SH_cont).
           rewrite PeanoNat.Nat.sub_diag in Temp.
           eapply Temp...
           rewrite H15. inversion H10...
-          apply nth_middle.
-        - eapply S_mov with
-            (d:=r1) (o:=val_direct_trans (var_val var) cur_stk_val)...
-          rewrite H15. inversion H10... apply nth_middle. }
+          apply nth_middle. }
       eapply multi_step.
       { eapply S_sfree with
           (n:=List.length (List.map run_cst_trans E1))...
         - cbn. rewrite H15. inversion H10...
-          destruct v as [|[|]];
+          destruct v as [|[]];
             rewrite Nat.add_comm,map_length;
             apply ins_verify with (n:=1).
         - rewrite app_length... }
@@ -2207,7 +1032,7 @@ Proof with super_a.
                  loc_w (cloc Clab_op 0)])
           (lsp:=L0) (pred_j:=4)...
         rewrite H15. inversion H10...
-        destruct v as [|[|]];
+        destruct v as [|[]];
           apply ins_verify with (n:=2). }
       eapply multi_step.
       { eapply S_pop with (reg:=r2)... }
@@ -2251,7 +1076,7 @@ Proof with super_a.
             rewrite app_length. inversion H22... 
           + rewrite <- app_assoc.
             inversion H28...
-            destruct v as [cst|[ind|str]]...
+            destruct v as [cst|[ind]]...
             rewrite <- map_nth with (d:=L.ns).
             rewrite app_nth1.
             inversion H10...
@@ -2274,9 +1099,9 @@ Proof with super_a.
     inversion H6...
     inversion H7...
     specialize H16 with
-      (L':=hloc_str L) (s':=s0) (H':=H1).
-    assert (Temp:(hloc_str L, stack s0) :: H1
-                 = (hloc_str L, stack s0) :: H1)...
+      (L':=hloc_num L) (s':=s0) (H':=H1).
+    assert (Temp:(hloc_num L, stack s0) :: H1
+                 = (hloc_num L, stack s0) :: H1)...
     apply H16 in Temp.
     unfold stk_points_to in Temp.
     rewrite rev_app_distr in Temp.
@@ -2292,7 +1117,7 @@ Proof with super_a.
         as cur_stk_val.
     esplit. esplit. split.
     + eapply multi_step.
-      { destruct v2 as [cst|[ind|var]].
+      { destruct v2 as [cst|[ind]].
         - eapply S_mov with
             (d:=r2) (o:=val_direct_trans cst cur_stk_val)...
           cbn. rewrite H15. inversion H10... apply nth_middle.
@@ -2301,18 +1126,15 @@ Proof with super_a.
           specialize Temp with
             (d:=r2) (load_off:=ind) (lst:=cur_stk_val)
             (reg_off:=List.length cur_stk_val)(s:=sp)
-            (H_stk_ld:=[]) (L:=hloc_str L_str)
-            (H_stk_ed:=(hloc_str L, stack s0)
+            (H_stk_ld:=[]) (L:=hloc_num L_str)
+            (H_stk_ed:=(hloc_num L, stack s0)
                          :: H1 ++ SH_cont).
           rewrite PeanoNat.Nat.sub_diag in Temp.
           eapply Temp...
           rewrite H15. inversion H10...
-          apply nth_middle.
-        - eapply S_mov with
-            (d:=r2) (o:=val_direct_trans (var_val var) cur_stk_val)...
-          rewrite H15. inversion H10... apply nth_middle. }
+          apply nth_middle. }
       eapply multi_step.
-      { destruct v1 as [cst|[ind|var]].
+      { destruct v1 as [cst|[ind]].
         - eapply S_mov with
             (d:=r1) (o:=val_direct_trans cst cur_stk_val)...
         - destruct Temp.
@@ -2324,9 +1146,7 @@ Proof with super_a.
           rewrite PeanoNat.Nat.sub_diag in Temp.
           eapply Temp...
           rewrite H15. inversion H10...
-          apply ins_verify with (n:=1).
-        - eapply S_mov with
-            (d:=r1) (o:=val_direct_trans (var_val var) cur_stk_val)... }
+          apply ins_verify with (n:=1). }
       eapply multi_step.
       { eapply S_call
           with (o:=wd_o (cloc raise_loc 0))...
@@ -2339,9 +1159,9 @@ Proof with super_a.
             (H_stk_ld:=[])
             (lst:=loc_w (cloc Clab (3 + List.length lst))
                     :: cur_stk_val)
-            (H_stk_ed:=(hloc_str L, stack s0) ::
+            (H_stk_ed:=(hloc_num L, stack s0) ::
                          H1 ++ SH_cont)...
-        destruct v1 as [|[|]]...
+        destruct v1 as [|[]]...
         inversion H8... rewrite app_nth1,
           map_nth with (d:=L.ns),H3...
         rewrite map_length.
@@ -2353,14 +1173,14 @@ Proof with super_a.
           (H_stk_ld:=[])
           (lst:=loc_w (cloc Clab (3 + List.length lst))
                   :: cur_stk_val)
-          (H_stk_ed:=(hloc_str L, stack s0)
+          (H_stk_ed:=(hloc_num L, stack s0)
                        :: H1 ++ SH_cont).
         5:{ subst. rewrite app_comm_cons.
             repeat (rewrite app_length).
             rewrite Nat.add_comm... }
         super_a. super_a.
         2:{ super_a. }
-        destruct v1 as [|[|]]...
+        destruct v1 as [|[]]...
         inversion H8... rewrite app_nth1,
           map_nth with (d:=L.ns),H3...
         rewrite map_length.
@@ -2383,7 +1203,7 @@ Proof with super_a.
           (o:=r4) (H_cont:=SH_cont) (H_stk_ed:=H1)
           (l:=cloc raise_loc 2)
           (H_stk_ld:=
-             [(hloc_str L_str,
+             [(hloc_num L_str,
                 stack (loc_w (cloc Clab (3 + Datatypes.length lst))
                          :: map run_cst_trans E1 ++ s ++
                          [loc_w (cloc handle_loc 10);
@@ -2407,9 +1227,9 @@ Proof with super_a.
       eapply multi_step.
       { eapply S_load_stk with
           (d:=r5) (s:=r1) (load_off:=3)
-          (H_stk_ld:=(hloc_str L, stack s0) :: H1)
+          (H_stk_ld:=(hloc_num L, stack s0) :: H1)
           (H_stk_ed:=SH_cont)...
-        destruct v1 as [|[|]]...
+        destruct v1 as [|[]]...
         inversion H8... rewrite app_nth1,
           map_nth with (d:=L.ns),H3...
         rewrite map_length.
@@ -2427,9 +1247,9 @@ Proof with super_a.
       eapply multi_step.
       { eapply S_load_stk with
           (d:=r1) (s:=r1) (load_off:=2)
-          (H_stk_ld:=(hloc_str L, stack (skipn 0 s0)) :: H1)
+          (H_stk_ld:=(hloc_num L, stack (skipn 0 s0)) :: H1)
           (H_stk_ed:=SH_cont)...
-        destruct v1 as [|[|]]...
+        destruct v1 as [|[]]...
         inversion H8... rewrite app_nth1,
           map_nth with (d:=L.ns),H3...
         rewrite map_length.
@@ -2472,7 +1292,7 @@ Proof with super_a.
         (lst:=[push r3;push r2;push r1])
         (SIlst:=func_term_trans 3 t1')
         (SH_cont:=
-           (hloc_str L_str,
+           (hloc_num L_str,
              stack (loc_w (cloc Clab (3 + Datatypes.length lst))
                       :: map run_cst_trans E1 ++ s ++
                       [loc_w (cloc handle_loc 10);
@@ -2498,15 +1318,15 @@ Proof with super_a.
         cbn.
         apply rel_env_context with
           (s_out:=s0)...
-        destruct v2 as [cst|[ind|str]]...
+        destruct v2 as [cst|[ind]]...
         rewrite <- map_nth with (d:=L.ns).
         rewrite app_nth1... inversion H10...
         rewrite List.map_length.
         inversion H3... inversion H25...
-        inversion H28...
+        inversion H27...
       * intros. inversion H13...
         inversion H26...
-      * cbn. destruct v1 as [|[|]]...
+      * cbn. destruct v1 as [|[]]...
         inversion H8... rewrite app_nth1,
           map_nth with (d:=L.ns),H3...
         2:{ rewrite map_length.
@@ -2557,13 +1377,8 @@ Proof with super_a.
     destruct L_k as [L_k_str].
     destruct L_new as [L_new].
     inversion H5;subst.
-    (*assert (Temp:forall {A} a b (l l': list A),
-               l' ++ a :: b :: l = l' ++ [a] ++ b :: l). {super_a.}
-    rewrite Temp, app_assoc in H7.*)
     apply eval_ctx_app_2_middle in H7.
     2:{super_a.} 2:{ super_a. }
-    (*rewrite app_comm_cons,Temp,app_assoc in H5.
-    apply eval_ctx_app_split in H5.*)
     destruct H7 as
       [s1 [s2 [H_ld [H_ed hyp]]]].
     destruct hyp as [hyp1 [hyp2 [hyp3 hyp4]]].
@@ -2573,7 +1388,6 @@ Proof with super_a.
     destruct hyp1 as [hyp1 _].
     inversion hyp1;subst.
     inversion H6;subst.
-    (*inversion H24.*)
     remember
       (map run_cst_trans E1 ++
          s_out) as cur_stk_val.
@@ -2584,14 +1398,9 @@ Proof with super_a.
         loc_w (hloc L_env 0);
         loc_w (cloc Clab_op 0)])
         as frm_stk.
-     (* l code loc
-        SH_tups
-        R36
-        H_stks
-        cur_stkh*)
     esplit. esplit. split.
     + eapply multi_step.
-      { destruct v2 as [cst|[ind|var]].
+      { destruct v2 as [cst|[ind]].
         - eapply S_mov with
             (d:=r2) (o:=val_direct_trans cst cur_stk_val)...
           cbn. rewrite H15. inversion H10... apply nth_middle.
@@ -2603,12 +1412,9 @@ Proof with super_a.
           rewrite PeanoNat.Nat.sub_diag in Tmp.
           eapply Tmp...
           + rewrite H15. inversion H10...
-            apply nth_middle.
-        - eapply S_mov with
-            (d:=r2) (o:=val_direct_trans (var_val var) cur_stk_val)...
-          rewrite H15. inversion H10... apply nth_middle. }
+            apply nth_middle. }
       eapply multi_step.
-      { destruct v1 as [cst|[ind|var]].
+      { destruct v1 as [cst|[ind]].
         - eapply S_mov with
             (d:=r1) (o:=val_direct_trans cst cur_stk_val)...
         - pose proof S_load_stk as Tmp.
@@ -2619,61 +1425,24 @@ Proof with super_a.
           rewrite PeanoNat.Nat.sub_diag in Tmp.
           eapply Tmp...
           + rewrite H15. inversion H10...
-            apply ins_verify with (n:=1).
-        - eapply S_mov with
-            (d:=r1) (o:=val_direct_trans (var_val var) cur_stk_val)... }
+            apply ins_verify with (n:=1). }
       eapply multi_step.
       { eapply S_call
           with (o:=wd_o (cloc raise_loc 0))...
         rewrite H15. inversion H10...
         apply ins_verify with (n:=2). }
       eapply multi_step.
-      { (*inversion hyp3.*)
-        unfold next_cloc.
-        Check S_load_stk. cbn.
+      { unfold next_cloc. cbn.
         eapply S_load_stk with
           (d:=r4) (s:=r1) (load_off:=0)
           (l:=cloc raise_loc 0)
-          (*R:=[(ip,loc_w (cloc raise_loc 0));
-               (sp,
-                 loc_w (hloc L (S (List.length
-                                     cur_stk_val))));
-               (r0,o0);
-               (r1,val_direct_trans v1
-                     (List.map run_cst_trans E1
-                        ++ s0 ++
-                        [loc_w (cloc handle_loc 10);
-                         loc_w (hloc L_prev (Datatypes.length s_prev));
-                         int_w 0; 
-                         loc_w (hloc L_env 0);
-                         loc_w (cloc Clab_op 0)]));
-               (r2,val_direct_trans v2
-                     (List.map run_cst_trans E1
-                        ++ s0 ++
-                        [loc_w (cloc handle_loc 10);
-                         loc_w (hloc L_prev (Datatypes.length s_prev));
-                         int_w 0; 
-                         loc_w (hloc L_env 0);
-                         loc_w (cloc Clab_op 0)]));
-               (r3,o3);
-               (r4,o4);
-               (r5,o5);(r6,o6)]*)
           (H_stk_ld:=
-             (hloc_str L,
+             (hloc_num L,
                stack (loc_w (cloc Clab (3 + List.length lst))
                         :: map run_cst_trans E1 ++ s_out))
-               :: H_ld(* ++
-               [(hloc_str L_str,
-                  stack
-                    (s0 ++
-                       [loc_w (cloc handle_loc 10);
-                        loc_w (hloc L_prev (Datatypes.length s_prev));
-                        int_w 0; 
-                        loc_w (hloc L_env 0);
-                        loc_w (cloc Clab_op 0)]))]*))
-          (lst:=s ++ frm_stk)
-          (*H_stk_ed:=H_ed ++ SH_cont*)...
-        - destruct v1 as [|[|]]...
+               :: H_ld)
+          (lst:=s ++ frm_stk)...
+        - destruct v1 as [|[]]...
           inversion H8... rewrite app_nth1,
             map_nth with (d:=L.ns),H2...
           rewrite map_length.
@@ -2684,14 +1453,12 @@ Proof with super_a.
       { eapply S_store_stk with
           (d:=r1) (load_off:=0) (o:=sp)
           (H_stk_ld:=
-             (hloc_str L,
+             (hloc_num L,
                stack (loc_w (cloc Clab (3 + List.length lst))
                         :: map run_cst_trans E1 ++ s_out))
                :: H_ld)
-          (L:=L_str)
-          (*lst:=s_md)
-          (H_stk_ed:=H_ed ++ SH_cont*)...
-        - destruct v1 as [|[|]]...
+          (L:=L_str)...
+        - destruct v1 as [|[]]...
           inversion H8... rewrite app_nth1,
             map_nth with (d:=L.ns),H2...
           rewrite map_length.
@@ -2699,43 +1466,23 @@ Proof with super_a.
           inversion H20... inversion H17...
         - repeat (rewrite <- app_assoc)...
         - rewrite app_length... }
-      (*rewrite <- H22.*)
       rewrite Nat.add_0_r.
       rewrite update_nth_split with
         (l2:=frm_stk).
-      2:{ super_a. } (*rewrite <- H26.*)
+      2:{ super_a. }
       inversion hyp2.
-      (*assert (hloc_str L0 = L_prev /\
-             s1 = s_prev).
-      { 
-
-        rewrite app_comm_cons in H5.
-        apply eval_ctx_app_split in H5.
-        destruct H5 as
-          [H_ld'' [H_ed' [hy1 [hy2 hy3]]]].
-        subst. inversion hy2;subst.
-        inversion H4;subst.
-        assert ((hloc_str L2,stack s2) :: H2
-                = (hloc_str L2,stack s2) :: H2);trysolve.
-        apply H7 in H1. unfold stk_points_to in H1.
-      }*)
-      
       eapply multi_step.
       { repeat (rewrite app_comm_cons).
         rewrite app_assoc.
-
-        Check S_mov_sp_to_cont.
-        
-        
         eapply S_mov_sp_to_cont with
           (o:=r4) (H_cont:=SH_cont) (H_stk_ed:=H_ed)
           (l:=cloc raise_loc 2)
           (H_stk_ld:=(*what we put to cont*)
-             (hloc_str L,
+             (hloc_num L,
                stack (loc_w (cloc Clab (3 + List.length lst))
                         :: map run_cst_trans E1 ++ s_out))
                :: H_ld ++
-               [(hloc_str L_str,
+               [(hloc_num L_str,
                   stack (s ++ [loc_w (cloc handle_loc 10);
                                 loc_w (hloc L
                                          (S (List.length (map run_cst_trans E1
@@ -2746,21 +1493,7 @@ Proof with super_a.
           (*top stack not in cont*)
           (L:=L_new)
           (lst:=s2)...
-        
-          (*H_stk_ld:=
-             [(hloc_str L_str,
-                stack (loc_w (cloc Clab (3 + Datatypes.length lst))
-                         :: map run_cst_trans E1 ++ s ++
-                         [loc_w (cloc handle_loc 10);
-                          loc_w (hloc L_str
-                                   (6 + (List.length (map run_cst_trans E1 ++ s))));
-                          int_w 0;
-                          loc_w (hloc L_env0 0); 
-                          loc_w (cloc Clab_op 0)]))])
-          (L:=L) (j:=List.length s0)
-          (lst:=s0*)
         - (*we placed L_prev s_prev in r4*)
-          (*rewrite app_comm_cons,Nat.add_0_r.*)
           rewrite <- rev_nth with (n:=3),
               rev_app_distr.
           2:{ repeat (rewrite app_length).
@@ -2774,18 +1507,17 @@ Proof with super_a.
           rewrite <- app_assoc... }
       rewrite Nat.sub_diag.
       eapply multi_step.
-      { Check S_load_stk.
-        eapply S_load_stk with
+      { eapply S_load_stk with
           (d:=r5) (s:=r1) (load_off:=3)
           (H_stk_ld:=
-             (hloc_str L_new, stack s2) :: H_ed
-               ++ (hloc_str L,
+             (hloc_num L_new, stack s2) :: H_ed
+               ++ (hloc_num L,
                  stack (loc_w (cloc Clab (3 + List.length lst))
                           :: map run_cst_trans E1 ++ s_out))
                :: H_ld)
           (L:=L_str)
           (H_stk_ed:=SH_cont)...
-        - destruct v1 as [|[|]]...
+        - destruct v1 as [|[]]...
           inversion H8...
           rewrite app_nth1,
             map_nth with (d:=L.ns),H2...
@@ -2806,13 +1538,13 @@ Proof with super_a.
       { cbn. eapply S_load_stk with
           (d:=r1) (s:=r1) (load_off:=2)
            (H_stk_ld:=
-             (hloc_str L_new, stack s2) :: H_ed
-               ++ (hloc_str L,
+             (hloc_num L_new, stack s2) :: H_ed
+               ++ (hloc_num L,
                  stack (loc_w (cloc Clab (3 + List.length lst))
                           :: map run_cst_trans E1 ++ s_out))
                :: H_ld)
           (H_stk_ed:=SH_cont)...
-        - destruct v1 as [|[|]]...
+        - destruct v1 as [|[]]...
           inversion H8... rewrite app_nth1,
             map_nth with (d:=L.ns),H2...
           rewrite map_length.
@@ -2872,8 +1604,7 @@ Proof with super_a.
           rewrite Nat.add_comm... }
       rewrite <- rev_nth with (n:=3),
           rev_app_distr.
-      2:{ (*rewrite <- H26.*)
-          repeat (rewrite app_length).
+      2:{ repeat (rewrite app_length).
           rewrite Nat.add_comm... }
       cbn.
       rewrite <- app_assoc.
@@ -2881,41 +1612,20 @@ Proof with super_a.
       apply rel_LS with
         (lst:=[push r3;push r2;push r1])
         (SIlst:=func_term_trans 3 t1')...
-        (*SH_stack:=
-           (hloc_str L_new,
-             stack
-               (loc_w (hloc L_env 0) ::
-                  val_direct_trans v2
-                  (map run_cst_trans E1 ++ s)
-                  :: loc_w (hloc L_k_str 0) :: s2)) :: H_ed).
-        (SH_cont:=
-           (hloc_str L,
-             stack (loc_w (cloc Clab (3 + Datatypes.length lst))
-                      :: map run_cst_trans E1 ++ s_out))
-             :: H_ld ++    
-             [(hloc_str L_str,
-             stack (s0 ++
-                      [loc_w (cloc handle_loc 10);
-                       loc_w (hloc L_out
-                                (S (List.length (map run_cst_trans E1 ++ s))));
-                       int_w 0;
-                       loc_w (hloc L_env 0); 
-                       loc_w (cloc Clab_op 0)]))]
-             ++ SH_cont*)
       * inversion H14... specialize H2 with
           (x:=c_lab Clab_op).
         rewrite H18 in H2. inversion H2...        
       * apply rel_env_context with
           (s_out:=s2)...
-        destruct v2 as [cst|[ind|str]]...
+        destruct v2 as [cst|[ind]]...
         rewrite <- map_nth with (d:=L.ns).
         rewrite app_nth1... inversion H10...
         rewrite List.map_length.
         inversion H2... inversion H17...
-        inversion H22...
+        inversion H21...
       * intros. inversion H13...
         inversion H20...
-      * destruct v1 as [|[|]]...
+      * destruct v1 as [|[]]...
         inversion H8... rewrite app_nth1,
           map_nth with (d:=L.ns),H2...
         2:{ rewrite map_length.
@@ -2937,12 +1647,10 @@ Proof with super_a.
                   int_w 0; 
                   loc_w (hloc L_env 0);
                   loc_w (cloc Clab_op 0)])...
-            Check rel_hdl_general.
             apply rel_hdl_general with
               (s_prev:=ns :: map run_cst_trans E1 ++ s_out).
           - inversion H11...
             rewrite app_comm_cons,app_assoc.
-            Check rel_hdl_stk_base.
             constructor...
             apply rel_frame with
               (lst:=lst ++ firstn 3 SIlst)
@@ -3023,7 +1731,7 @@ Proof with super_a.
       [s_prev_len_eq HeqL_prev].         
     esplit. esplit. split.
     + eapply multi_step.
-      { destruct v2 as [cst|[ind|var]].
+      { destruct v2 as [cst|[ind]].
         - eapply S_mov with
             (d:=r2) (o:=val_direct_trans cst cur_stk_val)...
           cbn. rewrite H15. inversion H10... apply nth_middle.
@@ -3035,12 +1743,9 @@ Proof with super_a.
           rewrite PeanoNat.Nat.sub_diag in Tmp.
           eapply Tmp...
           + rewrite H15. inversion H10...
-            apply nth_middle.
-        - eapply S_mov with
-            (d:=r2) (o:=val_direct_trans (var_val var) cur_stk_val)...
-          rewrite H15. inversion H10... apply nth_middle. }
+            apply nth_middle. }
       eapply multi_step.
-      { destruct v1 as [cst|[ind|var]].
+      { destruct v1 as [cst|[ind]].
         - eapply S_mov with
             (d:=r1) (o:=val_direct_trans cst cur_stk_val)...
         - pose proof S_load_stk as Tmp.
@@ -3051,26 +1756,23 @@ Proof with super_a.
           rewrite PeanoNat.Nat.sub_diag in Tmp.
           eapply Tmp...
           + rewrite H15. inversion H10...
-            apply ins_verify with (n:=1).
-        - eapply S_mov with
-            (d:=r1) (o:=val_direct_trans (var_val var) cur_stk_val)... }
+            apply ins_verify with (n:=1). }
       eapply multi_step.
       { eapply S_call
           with (o:=wd_o (cloc resume_loc 0))...
         rewrite H15. inversion H10...
         apply ins_verify with (n:=2). }
-     (**)
       eapply multi_step.
       { eapply S_load_tup_c with
           (d:=r3) (s:=r1) (off:=0)...
-        - destruct v1 as [|[|]]...
+        - destruct v1 as [|[]]...
           inversion H4... rewrite app_nth1,
             map_nth with (d:=L.ns),H2...
           rewrite map_length.
           inversion H10... inversion H28...
           inversion H33... inversion H32...
         - specialize hyp5 with
-            (L:=hloc_str L_k_str).
+            (L:=hloc_num L_k_str).
           inversion hyp5.
           + unfold th_update in H1.
             rewrite h_eqb_refl in H1...
@@ -3081,14 +1783,14 @@ Proof with super_a.
       eapply multi_step.
       { eapply S_store_c_ns with
           (d:=r1)...
-        - destruct v1 as [|[|]]...
+        - destruct v1 as [|[]]...
           inversion H4... rewrite app_nth1,
             map_nth with (d:=L.ns),H2...
           rewrite map_length.
           inversion H10... inversion H28...
           inversion H33... inversion H32...
         - specialize hyp5 with
-            (L:=hloc_str L_k_str).
+            (L:=hloc_num L_k_str).
           inversion hyp5.
           + unfold th_update in H1.
             rewrite h_eqb_refl in H1...
@@ -3115,7 +1817,6 @@ Proof with super_a.
       eapply multi_step.
       { eapply S_mov with
           (d:=r1) (o:=r2)... }
-      (**)
       rewrite Nat.add_0_r.
       rewrite <- Heqstk_last.
       rewrite update_nth_split.
@@ -3124,8 +1825,7 @@ Proof with super_a.
         rev_app_distr.
       2:{ rewrite app_length,Nat.add_comm... }
       eapply multi_step.
-      { Check S_mov_sp_from_cont.
-        rewrite app_comm_cons,<-app_assoc.
+      { rewrite app_comm_cons,<-app_assoc.
         eapply S_mov_sp_from_cont with
           (o:=r4) (H_cont':=[])
           (lst:=update_nth (List.length s_last - 4) s_last
@@ -3171,7 +1871,7 @@ Proof with super_a.
         -- inversion H5...
            { inversion H35...
              rewrite app_comm_cons,app_assoc.
-             constructor... Check rel_frame.
+             constructor...
              apply rel_frame with
                (Ilst:=push r1 :: func_term_trans (List.length (L.ns :: E1)) t)
                (lst:=lst ++ firstn 3 SIlst);trysolve;
@@ -3201,7 +1901,7 @@ Proof with super_a.
            rewrite List.map_length...
       * unfold th_update in hyp5.
         rewrite update_comp_cancel...
-        2:{ specialize hyp5 with (hloc_str L_k_str).
+        2:{ specialize hyp5 with (hloc_num L_k_str).
             destruct hyp5 as [hyp5|]...
             rewrite h_eqb_refl in hyp5... }
         apply cont_heap_app;trysolve.
@@ -3261,7 +1961,7 @@ Proof with super_a.
       [s_prev_len_eq HeqL_prev].         
     esplit. esplit. split.
     + eapply multi_step.
-      { destruct v2 as [cst|[ind|var]].
+      { destruct v2 as [cst|[ind]].
         - eapply S_mov with
             (d:=r2) (o:=val_direct_trans cst cur_stk_val)...
           cbn. rewrite H15. inversion H10... apply nth_middle.
@@ -3273,12 +1973,9 @@ Proof with super_a.
           rewrite PeanoNat.Nat.sub_diag in Tmp.
           eapply Tmp...
           + rewrite H15. inversion H10...
-            apply nth_middle.
-        - eapply S_mov with
-            (d:=r2) (o:=val_direct_trans (var_val var) cur_stk_val)...
-          rewrite H15. inversion H10... apply nth_middle. }
+            apply nth_middle. }
       eapply multi_step.
-      { destruct v1 as [cst|[ind|var]].
+      { destruct v1 as [cst|[ind]].
         - eapply S_mov with
             (d:=r1) (o:=val_direct_trans cst cur_stk_val)...
         - pose proof S_load_stk as Tmp.
@@ -3289,26 +1986,23 @@ Proof with super_a.
           rewrite PeanoNat.Nat.sub_diag in Tmp.
           eapply Tmp...
           + rewrite H15. inversion H10...
-            apply ins_verify with (n:=1).
-        - eapply S_mov with
-            (d:=r1) (o:=val_direct_trans (var_val var) cur_stk_val)... }
+            apply ins_verify with (n:=1). }
       eapply multi_step.
       { eapply S_call
           with (o:=wd_o (cloc resume_loc 0))...
         rewrite H15. inversion H10...
         apply ins_verify with (n:=2). }
-      (**)
       eapply multi_step.
       { eapply S_load_tup_c with
           (d:=r3) (s:=r1) (off:=0)...
-        - destruct v1 as [|[|]]...
+        - destruct v1 as [|[]]...
           inversion H6... rewrite app_nth1,
             map_nth with (d:=L.ns),H17...
           rewrite map_length.
           inversion H10... inversion H32...
           inversion H37... inversion H36...
         - specialize hyp5 with
-            (L:=hloc_str L_k_str).
+            (L:=hloc_num L_k_str).
           inversion hyp5.
           + unfold th_update in H2.
             rewrite h_eqb_refl in H2...
@@ -3319,14 +2013,14 @@ Proof with super_a.
       eapply multi_step.
       { eapply S_store_c_ns with
           (d:=r1)...
-        - destruct v1 as [|[|]]...
+        - destruct v1 as [|[]]...
           inversion H6... rewrite app_nth1,
             map_nth with (d:=L.ns),H17...
           rewrite map_length.
           inversion H10... inversion H32...
           inversion H37... inversion H36...
         - specialize hyp5 with
-            (L:=hloc_str L_k_str).
+            (L:=hloc_num L_k_str).
           inversion hyp5.
           + unfold th_update in H2.
             rewrite h_eqb_refl in H2...
@@ -3334,7 +2028,6 @@ Proof with super_a.
             rewrite H2.
             unfold th_update.
             rewrite h_eqb_refl... }
-      (**)
       eapply multi_step.
       { rewrite <- app_assoc,
           <- app_comm_cons.        
@@ -3345,7 +2038,7 @@ Proof with super_a.
                stack (loc_w (cloc Clab (3 + List.length lst))
                         :: map run_cst_trans E1 ++ s_out))
                :: H_stack ++ SH_cont_ld
-               ++ (hloc_str L,stack s) :: H_one_cont_ld')...
+               ++ (hloc_num L,stack s) :: H_one_cont_ld')...
         repeat (rewrite <- app_assoc)... }
       eapply multi_step.
       { eapply S_store_stk with
@@ -3355,14 +2048,13 @@ Proof with super_a.
                stack (loc_w (cloc Clab (3 + List.length lst))
                         :: map run_cst_trans E1 ++ s_out))
                :: H_stack ++ SH_cont_ld
-               ++ (hloc_str L,stack s) :: H_one_cont_ld')...
+               ++ (hloc_num L,stack s) :: H_one_cont_ld')...
         - repeat (rewrite <- app_assoc)...
         - rewrite app_length,
             Nat.add_comm... }
       eapply multi_step.
       { eapply S_mov with
           (d:=r1) (o:=r2)... }
-      (**)
       rewrite Nat.add_0_r.
       rewrite <- Heqstk_last.
       rewrite update_nth_split.
@@ -3372,13 +2064,13 @@ Proof with super_a.
       2:{ rewrite app_length,Nat.add_comm... }
       
       eapply multi_step.
-      { cbn. Check S_mov_sp_from_cont.
+      { cbn.
         rewrite <-app_assoc,app_comm_cons.
         eapply S_mov_sp_from_cont with
           (o:=r4) (lst:=s)
           (H_cont':=
              H_one_cont_ld' ++
-               [(hloc_str L_cont,
+               [(hloc_num L_cont,
                   stack
                     (update_nth (List.length s_last - 4)
                        s_last
@@ -3487,7 +2179,7 @@ Proof with super_a.
            rewrite List.map_length...
       * unfold th_update in hyp5.
         rewrite update_comp_cancel...
-        2:{ specialize hyp5 with (hloc_str L_k_str).
+        2:{ specialize hyp5 with (hloc_num L_k_str).
             destruct hyp5 as [hyp5|]...
             rewrite h_eqb_refl in hyp5... }
         apply cont_heap_app;trysolve.
@@ -3500,34 +2192,3 @@ Proof with super_a.
       * destruct Ilst...
         rewrite app_length...
 Qed.
-                   
-             
-   
-(*other things
-0. changes in lexi heaps e.g. assignment
-1. handler related stuff
-2. relating data heap
-3. relating hdl-led-ctx*)
-
-
-(*
-All changes made
-malloc rule's register should be r_d in resulting state
-newref's translation s hould be malloc r2 n rather than i
-
-simplifications can be done:
-sfree after function call is just size of environment,
-      no need to compute numlet
- *)
-(* new changes after paper submitted
-0. change definition of relating frames
-1. passes parameter C_mem all the way down to frame relation
-2. added well-formed ness for rel_ins rather than at LS_rel
-3. handler relation should also store return location
-4. handler rule for lexi should swap order of env and L
-   (this actually doesn't matter for paper proof since
-    paper proof uses named variables)*)
-
-
-
-
