README.md
@@ -1,10 +1,17 @@
-Coq formalization of the syntax and operational semantics of LEXI and SALT, the compiler from LEXI to SALT, and the proof of correctness of compiler.
+# Lexa - A Programming Language Supporting Compiled Lexical Scoped Effect Handlers
 
-Lexi.v contains the abstract syntax and operational semantics of Lexi, the IR supporting lexical scoped effect handlers.
+This project contains the Coq formalization of the syntax and operational semantics of LEXA and SALT, the compiler from LEXA to SALT, and the proof of correctness of compiler.
 
-Salt.v contains the abstract syntax and operational semantics of Salt, the assembly language.
-LexiToSalt.v defines translation/compiler from Lexi to Salt.
+## Overview of Files
 
-RelConfig.v defines predicate relating the runtime configurations of Lexi and Salt.
+- Lexa.v contains the abstract syntax and operational semantics of Lexa, the high level language supporting lexical scoped effect handlers.
+
+- Salt.v contains the abstract syntax and operational semantics of Salt, an assembly language that Lexa compiles to.
+
+- LexaToSalt.v defines a translation function that takes in Lexa code and produces Salt code. It is essentially a compiler, except that its input is already Lexa abstract syntax and not strings.
+
+- RelConfig.v defines a predicate relating the runtime configurations of Lexa and Salt, which will be used in SimProof.v for the simulation proof of the compiler's correctness.
+
+- Infrastructure.v contains some lemmas used in the proofs in SimProof.v, and some simple tactics.
 
 SimProof.v contains the simulation proof for the correctness of translation.
